<?xml version="1.0"?>
<rdf:RDF xmlns="https://w3id.org/rdo#"
     xml:base="https://w3id.org/rdo"
     xmlns:dc="http://purl.org/dc/elements/1.1/"
     xmlns:ns="http://www.w3.org/2003/06/sw-vocab-status/ns#"
     xmlns:owl="http://www.w3.org/2002/07/owl#"
     xmlns:rdf="http://www.w3.org/1999/02/22-rdf-syntax-ns#"
     xmlns:xml="http://www.w3.org/XML/1998/namespace"
     xmlns:xsd="http://www.w3.org/2001/XMLSchema#"
     xmlns:dcam="http://purl.org/dc/dcam/"
     xmlns:rdfs="http://www.w3.org/2000/01/rdf-schema#"
     xmlns:vann="http://purl.org/vocab/vann/"
     xmlns:terms="http://purl.org/dc/terms/"
     xmlns:schema="http://schema.org/#"
     xmlns:sw-vocab-status="http://www.w3.org/2003/06/sw-vocab-status/">
    <owl:Ontology rdf:about="https://w3id.org/rdo">
        <owl:versionIRI rdf:resource="https://w3id.org/rdo/0.5"/>
        <owl:imports rdf:resource="http://purl.org/spar/foaf"/>
        <owl:imports rdf:resource="https://pi.pauwel.be/voc/buildingelement"/>
        <owl:imports rdf:resource="https://w3id.org/dot/0.8"/>
        <dc:publisher>Cyberbuild, University of Edinburgh</dc:publisher>
        <terms:abstract>This ontology provides a semantic framework for representing roof condition inspection information, including roofs and roof pitches, inspections, orthophotos, and image-derived defect observations. It is designed to support structured documentation, querying, and interoperability within digital twin–based workflows for roof condition monitoring and maintenance, particularly in the context of existing and heritage buildings.</terms:abstract>
        <terms:created rdf:datatype="http://www.w3.org/2000/01/rdf-schema#Literal">2026-02-06</terms:created>
        <terms:creator>Frederic Bosche, University of Edinburgh</terms:creator>
        <terms:creator>Jiajun Li, University of Edinburgh</terms:creator>
        <terms:description>This ontology provides a semantic framework for representing roof condition inspection information, including roofs and roof pitches, inspections, orthophotos, and image-derived defect observations. It is designed to support structured documentation, querying, and interoperability within digital twin–based workflows for roof condition monitoring and maintenance, particularly in the context of existing and heritage buildings.</terms:description>
        <terms:license>https://creativecommons.org/licenses/by/4.0/</terms:license>
        <terms:title>Roof Damage Ontology</terms:title>
        <vann:preferredNamespacePrefix>rdo</vann:preferredNamespacePrefix>
        <vann:preferredNamespaceUri>https://w3id.org/rdo#</vann:preferredNamespaceUri>
        <rdfs:comment>This ontology was developed with support from Historic Environment Scotland (HES) and the Engineering and Physical Sciences Research Council (EPSRC), and informed by collaboration with domain experts in heritage roof inspection and maintenance.</rdfs:comment>
        <owl:versionInfo rdf:datatype="http://www.w3.org/2001/XMLSchema#decimal">0.5</owl:versionInfo>
    </owl:Ontology>
    


    <!-- 
    ///////////////////////////////////////////////////////////////////////////////////////
    //
    // Annotation properties
    //
    ///////////////////////////////////////////////////////////////////////////////////////
     -->


    


    <!-- http://purl.org/dc/dcam/domainIncludes -->


    <owl:AnnotationProperty rdf:about="http://purl.org/dc/dcam/domainIncludes"/>
    


    <!-- http://purl.org/dc/dcam/rangeIncludes -->


    <owl:AnnotationProperty rdf:about="http://purl.org/dc/dcam/rangeIncludes"/>
    


    <!-- http://purl.org/dc/elements/1.1/contributor -->


    <owl:AnnotationProperty rdf:about="http://purl.org/dc/elements/1.1/contributor"/>
    


    <!-- http://purl.org/dc/elements/1.1/coverage -->


    <owl:AnnotationProperty rdf:about="http://purl.org/dc/elements/1.1/coverage"/>
    


    <!-- http://purl.org/dc/elements/1.1/creator -->


    <owl:AnnotationProperty rdf:about="http://purl.org/dc/elements/1.1/creator"/>
    


    <!-- http://purl.org/dc/elements/1.1/date -->


    <owl:AnnotationProperty rdf:about="http://purl.org/dc/elements/1.1/date"/>
    


    <!-- http://purl.org/dc/elements/1.1/format -->


    <owl:AnnotationProperty rdf:about="http://purl.org/dc/elements/1.1/format"/>
    


    <!-- http://purl.org/dc/elements/1.1/identifier -->


    <owl:AnnotationProperty rdf:about="http://purl.org/dc/elements/1.1/identifier"/>
    


    <!-- http://purl.org/dc/elements/1.1/language -->


    <owl:AnnotationProperty rdf:about="http://purl.org/dc/elements/1.1/language"/>
    


    <!-- http://purl.org/dc/elements/1.1/publisher -->


    <owl:AnnotationProperty rdf:about="http://purl.org/dc/elements/1.1/publisher"/>
    


    <!-- http://purl.org/dc/elements/1.1/relation -->


    <owl:AnnotationProperty rdf:about="http://purl.org/dc/elements/1.1/relation"/>
    


    <!-- http://purl.org/dc/elements/1.1/rights -->


    <owl:AnnotationProperty rdf:about="http://purl.org/dc/elements/1.1/rights"/>
    


    <!-- http://purl.org/dc/elements/1.1/source -->


    <owl:AnnotationProperty rdf:about="http://purl.org/dc/elements/1.1/source"/>
    


    <!-- http://purl.org/dc/elements/1.1/subject -->


    <owl:AnnotationProperty rdf:about="http://purl.org/dc/elements/1.1/subject"/>
    


    <!-- http://purl.org/dc/elements/1.1/type -->


    <owl:AnnotationProperty rdf:about="http://purl.org/dc/elements/1.1/type"/>
    


    <!-- http://purl.org/dc/terms/abstract -->


    <owl:AnnotationProperty rdf:about="http://purl.org/dc/terms/abstract">
        <rdfs:subPropertyOf rdf:resource="http://purl.org/dc/elements/1.1/description"/>
        <rdfs:subPropertyOf rdf:resource="http://purl.org/dc/terms/description"/>
    </owl:AnnotationProperty>
    


    <!-- http://purl.org/dc/terms/accessRights -->


    <owl:AnnotationProperty rdf:about="http://purl.org/dc/terms/accessRights">
        <rdfs:subPropertyOf rdf:resource="http://purl.org/dc/elements/1.1/rights"/>
        <rdfs:subPropertyOf rdf:resource="http://purl.org/dc/terms/rights"/>
    </owl:AnnotationProperty>
    


    <!-- http://purl.org/dc/terms/accrualMethod -->


    <owl:AnnotationProperty rdf:about="http://purl.org/dc/terms/accrualMethod">
        <rdfs:domain rdf:resource="http://purl.org/dc/dcmitype/Collection"/>
    </owl:AnnotationProperty>
    


    <!-- http://purl.org/dc/terms/accrualPeriodicity -->


    <owl:AnnotationProperty rdf:about="http://purl.org/dc/terms/accrualPeriodicity">
        <rdfs:domain rdf:resource="http://purl.org/dc/dcmitype/Collection"/>
    </owl:AnnotationProperty>
    


    <!-- http://purl.org/dc/terms/accrualPolicy -->


    <owl:AnnotationProperty rdf:about="http://purl.org/dc/terms/accrualPolicy">
        <rdfs:domain rdf:resource="http://purl.org/dc/dcmitype/Collection"/>
    </owl:AnnotationProperty>
    


    <!-- http://purl.org/dc/terms/alternative -->


    <owl:AnnotationProperty rdf:about="http://purl.org/dc/terms/alternative">
        <rdfs:subPropertyOf rdf:resource="http://purl.org/dc/elements/1.1/title"/>
    </owl:AnnotationProperty>
    


    <!-- http://purl.org/dc/terms/audience -->


    <owl:AnnotationProperty rdf:about="http://purl.org/dc/terms/audience"/>
    


    <!-- http://purl.org/dc/terms/available -->


    <owl:AnnotationProperty rdf:about="http://purl.org/dc/terms/available">
        <rdfs:subPropertyOf rdf:resource="http://purl.org/dc/elements/1.1/date"/>
    </owl:AnnotationProperty>
    


    <!-- http://purl.org/dc/terms/bibliographicCitation -->


    <owl:AnnotationProperty rdf:about="http://purl.org/dc/terms/bibliographicCitation">
        <rdfs:subPropertyOf rdf:resource="http://purl.org/dc/elements/1.1/identifier"/>
    </owl:AnnotationProperty>
    


    <!-- http://purl.org/dc/terms/conformsTo -->


    <owl:AnnotationProperty rdf:about="http://purl.org/dc/terms/conformsTo">
        <rdfs:subPropertyOf rdf:resource="http://purl.org/dc/elements/1.1/relation"/>
        <rdfs:subPropertyOf rdf:resource="http://purl.org/dc/terms/relation"/>
    </owl:AnnotationProperty>
    


    <!-- http://purl.org/dc/terms/contributor -->


    <rdf:Description rdf:about="http://purl.org/dc/terms/contributor">
        <rdfs:subPropertyOf rdf:resource="http://purl.org/dc/elements/1.1/contributor"/>
    </rdf:Description>
    


    <!-- http://purl.org/dc/terms/coverage -->


    <owl:AnnotationProperty rdf:about="http://purl.org/dc/terms/coverage">
        <rdfs:subPropertyOf rdf:resource="http://purl.org/dc/elements/1.1/coverage"/>
    </owl:AnnotationProperty>
    


    <!-- http://purl.org/dc/terms/created -->


    <owl:AnnotationProperty rdf:about="http://purl.org/dc/terms/created">
        <rdfs:subPropertyOf rdf:resource="http://purl.org/dc/elements/1.1/date"/>
    </owl:AnnotationProperty>
    


    <!-- http://purl.org/dc/terms/creator -->


    <rdf:Description rdf:about="http://purl.org/dc/terms/creator">
        <rdfs:subPropertyOf rdf:resource="http://purl.org/dc/elements/1.1/creator"/>
        <rdfs:subPropertyOf rdf:resource="http://purl.org/dc/terms/contributor"/>
    </rdf:Description>
    


    <!-- http://purl.org/dc/terms/date -->


    <rdf:Description rdf:about="http://purl.org/dc/terms/date">
        <rdfs:subPropertyOf rdf:resource="http://purl.org/dc/elements/1.1/date"/>
    </rdf:Description>
    


    <!-- http://purl.org/dc/terms/dateAccepted -->


    <owl:AnnotationProperty rdf:about="http://purl.org/dc/terms/dateAccepted">
        <rdfs:subPropertyOf rdf:resource="http://purl.org/dc/elements/1.1/date"/>
    </owl:AnnotationProperty>
    


    <!-- http://purl.org/dc/terms/dateCopyrighted -->


    <owl:AnnotationProperty rdf:about="http://purl.org/dc/terms/dateCopyrighted">
        <rdfs:subPropertyOf rdf:resource="http://purl.org/dc/elements/1.1/date"/>
    </owl:AnnotationProperty>
    


    <!-- http://purl.org/dc/terms/dateSubmitted -->


    <owl:AnnotationProperty rdf:about="http://purl.org/dc/terms/dateSubmitted">
        <rdfs:subPropertyOf rdf:resource="http://purl.org/dc/elements/1.1/date"/>
    </owl:AnnotationProperty>
    


    <!-- http://purl.org/dc/terms/description -->


    <rdf:Description rdf:about="http://purl.org/dc/terms/description">
        <rdfs:subPropertyOf rdf:resource="http://purl.org/dc/elements/1.1/description"/>
    </rdf:Description>
    


    <!-- http://purl.org/dc/terms/educationLevel -->


    <owl:AnnotationProperty rdf:about="http://purl.org/dc/terms/educationLevel">
        <rdfs:subPropertyOf rdf:resource="http://purl.org/dc/terms/audience"/>
    </owl:AnnotationProperty>
    


    <!-- http://purl.org/dc/terms/extent -->


    <owl:AnnotationProperty rdf:about="http://purl.org/dc/terms/extent">
        <rdfs:subPropertyOf rdf:resource="http://purl.org/dc/elements/1.1/format"/>
        <rdfs:subPropertyOf rdf:resource="http://purl.org/dc/terms/format"/>
    </owl:AnnotationProperty>
    


    <!-- http://purl.org/dc/terms/format -->


    <rdf:Description rdf:about="http://purl.org/dc/terms/format">
        <rdfs:subPropertyOf rdf:resource="http://purl.org/dc/elements/1.1/format"/>
    </rdf:Description>
    


    <!-- http://purl.org/dc/terms/hasFormat -->


    <owl:AnnotationProperty rdf:about="http://purl.org/dc/terms/hasFormat">
        <rdfs:subPropertyOf rdf:resource="http://purl.org/dc/elements/1.1/relation"/>
        <rdfs:subPropertyOf rdf:resource="http://purl.org/dc/terms/relation"/>
    </owl:AnnotationProperty>
    


    <!-- http://purl.org/dc/terms/hasPart -->


    <owl:AnnotationProperty rdf:about="http://purl.org/dc/terms/hasPart">
        <rdfs:subPropertyOf rdf:resource="http://purl.org/dc/elements/1.1/relation"/>
        <rdfs:subPropertyOf rdf:resource="http://purl.org/dc/terms/relation"/>
    </owl:AnnotationProperty>
    


    <!-- http://purl.org/dc/terms/hasVersion -->


    <owl:AnnotationProperty rdf:about="http://purl.org/dc/terms/hasVersion">
        <rdfs:subPropertyOf rdf:resource="http://purl.org/dc/elements/1.1/relation"/>
        <rdfs:subPropertyOf rdf:resource="http://purl.org/dc/terms/relation"/>
    </owl:AnnotationProperty>
    


    <!-- http://purl.org/dc/terms/identifier -->


    <owl:AnnotationProperty rdf:about="http://purl.org/dc/terms/identifier">
        <rdfs:subPropertyOf rdf:resource="http://purl.org/dc/elements/1.1/identifier"/>
    </owl:AnnotationProperty>
    


    <!-- http://purl.org/dc/terms/isFormatOf -->


    <owl:AnnotationProperty rdf:about="http://purl.org/dc/terms/isFormatOf">
        <rdfs:subPropertyOf rdf:resource="http://purl.org/dc/elements/1.1/relation"/>
        <rdfs:subPropertyOf rdf:resource="http://purl.org/dc/terms/relation"/>
    </owl:AnnotationProperty>
    


    <!-- http://purl.org/dc/terms/isPartOf -->


    <owl:AnnotationProperty rdf:about="http://purl.org/dc/terms/isPartOf">
        <rdfs:subPropertyOf rdf:resource="http://purl.org/dc/elements/1.1/relation"/>
        <rdfs:subPropertyOf rdf:resource="http://purl.org/dc/terms/relation"/>
    </owl:AnnotationProperty>
    


    <!-- http://purl.org/dc/terms/isReferencedBy -->


    <owl:AnnotationProperty rdf:about="http://purl.org/dc/terms/isReferencedBy">
        <rdfs:subPropertyOf rdf:resource="http://purl.org/dc/elements/1.1/relation"/>
        <rdfs:subPropertyOf rdf:resource="http://purl.org/dc/terms/relation"/>
    </owl:AnnotationProperty>
    


    <!-- http://purl.org/dc/terms/isReplacedBy -->


    <owl:AnnotationProperty rdf:about="http://purl.org/dc/terms/isReplacedBy">
        <rdfs:subPropertyOf rdf:resource="http://purl.org/dc/elements/1.1/relation"/>
        <rdfs:subPropertyOf rdf:resource="http://purl.org/dc/terms/relation"/>
    </owl:AnnotationProperty>
    


    <!-- http://purl.org/dc/terms/isRequiredBy -->


    <owl:AnnotationProperty rdf:about="http://purl.org/dc/terms/isRequiredBy">
        <rdfs:subPropertyOf rdf:resource="http://purl.org/dc/elements/1.1/relation"/>
        <rdfs:subPropertyOf rdf:resource="http://purl.org/dc/terms/relation"/>
    </owl:AnnotationProperty>
    


    <!-- http://purl.org/dc/terms/isVersionOf -->


    <owl:AnnotationProperty rdf:about="http://purl.org/dc/terms/isVersionOf">
        <rdfs:subPropertyOf rdf:resource="http://purl.org/dc/elements/1.1/relation"/>
        <rdfs:subPropertyOf rdf:resource="http://purl.org/dc/terms/relation"/>
    </owl:AnnotationProperty>
    


    <!-- http://purl.org/dc/terms/issued -->


    <rdf:Description rdf:about="http://purl.org/dc/terms/issued">
        <rdfs:subPropertyOf rdf:resource="http://purl.org/dc/elements/1.1/date"/>
    </rdf:Description>
    


    <!-- http://purl.org/dc/terms/language -->


    <rdf:Description rdf:about="http://purl.org/dc/terms/language">
        <rdfs:subPropertyOf rdf:resource="http://purl.org/dc/elements/1.1/language"/>
    </rdf:Description>
    


    <!-- http://purl.org/dc/terms/license -->


    <rdf:Description rdf:about="http://purl.org/dc/terms/license">
        <rdfs:subPropertyOf rdf:resource="http://purl.org/dc/elements/1.1/rights"/>
        <rdfs:subPropertyOf rdf:resource="http://purl.org/dc/terms/rights"/>
    </rdf:Description>
    


    <!-- http://purl.org/dc/terms/mediator -->


    <owl:AnnotationProperty rdf:about="http://purl.org/dc/terms/mediator">
        <rdfs:subPropertyOf rdf:resource="http://purl.org/dc/terms/audience"/>
    </owl:AnnotationProperty>
    


    <!-- http://purl.org/dc/terms/medium -->


    <owl:AnnotationProperty rdf:about="http://purl.org/dc/terms/medium">
        <rdfs:subPropertyOf rdf:resource="http://purl.org/dc/elements/1.1/format"/>
        <rdfs:subPropertyOf rdf:resource="http://purl.org/dc/terms/format"/>
    </owl:AnnotationProperty>
    


    <!-- http://purl.org/dc/terms/modified -->


    <rdf:Description rdf:about="http://purl.org/dc/terms/modified">
        <rdfs:subPropertyOf rdf:resource="http://purl.org/dc/elements/1.1/date"/>
    </rdf:Description>
    


    <!-- http://purl.org/dc/terms/publisher -->


    <rdf:Description rdf:about="http://purl.org/dc/terms/publisher">
        <rdfs:subPropertyOf rdf:resource="http://purl.org/dc/elements/1.1/publisher"/>
    </rdf:Description>
    


    <!-- http://purl.org/dc/terms/references -->


    <owl:AnnotationProperty rdf:about="http://purl.org/dc/terms/references">
        <rdfs:subPropertyOf rdf:resource="http://purl.org/dc/elements/1.1/relation"/>
        <rdfs:subPropertyOf rdf:resource="http://purl.org/dc/terms/relation"/>
    </owl:AnnotationProperty>
    


    <!-- http://purl.org/dc/terms/relation -->


    <owl:AnnotationProperty rdf:about="http://purl.org/dc/terms/relation">
        <rdfs:subPropertyOf rdf:resource="http://purl.org/dc/elements/1.1/relation"/>
    </owl:AnnotationProperty>
    


    <!-- http://purl.org/dc/terms/replaces -->


    <owl:AnnotationProperty rdf:about="http://purl.org/dc/terms/replaces">
        <rdfs:subPropertyOf rdf:resource="http://purl.org/dc/elements/1.1/relation"/>
        <rdfs:subPropertyOf rdf:resource="http://purl.org/dc/terms/relation"/>
    </owl:AnnotationProperty>
    


    <!-- http://purl.org/dc/terms/requires -->


    <owl:AnnotationProperty rdf:about="http://purl.org/dc/terms/requires">
        <rdfs:subPropertyOf rdf:resource="http://purl.org/dc/elements/1.1/relation"/>
        <rdfs:subPropertyOf rdf:resource="http://purl.org/dc/terms/relation"/>
    </owl:AnnotationProperty>
    


    <!-- http://purl.org/dc/terms/rights -->


    <owl:AnnotationProperty rdf:about="http://purl.org/dc/terms/rights">
        <rdfs:subPropertyOf rdf:resource="http://purl.org/dc/elements/1.1/rights"/>
    </owl:AnnotationProperty>
    


    <!-- http://purl.org/dc/terms/source -->


    <owl:AnnotationProperty rdf:about="http://purl.org/dc/terms/source">
        <rdfs:subPropertyOf rdf:resource="http://purl.org/dc/elements/1.1/source"/>
        <rdfs:subPropertyOf rdf:resource="http://purl.org/dc/terms/relation"/>
    </owl:AnnotationProperty>
    


    <!-- http://purl.org/dc/terms/spatial -->


    <owl:AnnotationProperty rdf:about="http://purl.org/dc/terms/spatial">
        <rdfs:subPropertyOf rdf:resource="http://purl.org/dc/elements/1.1/coverage"/>
        <rdfs:subPropertyOf rdf:resource="http://purl.org/dc/terms/coverage"/>
    </owl:AnnotationProperty>
    


    <!-- http://purl.org/dc/terms/subject -->


    <owl:AnnotationProperty rdf:about="http://purl.org/dc/terms/subject">
        <rdfs:subPropertyOf rdf:resource="http://purl.org/dc/elements/1.1/subject"/>
    </owl:AnnotationProperty>
    


    <!-- http://purl.org/dc/terms/tableOfContents -->


    <owl:AnnotationProperty rdf:about="http://purl.org/dc/terms/tableOfContents">
        <rdfs:subPropertyOf rdf:resource="http://purl.org/dc/elements/1.1/description"/>
        <rdfs:subPropertyOf rdf:resource="http://purl.org/dc/terms/description"/>
    </owl:AnnotationProperty>
    


    <!-- http://purl.org/dc/terms/temporal -->


    <owl:AnnotationProperty rdf:about="http://purl.org/dc/terms/temporal">
        <rdfs:subPropertyOf rdf:resource="http://purl.org/dc/elements/1.1/coverage"/>
        <rdfs:subPropertyOf rdf:resource="http://purl.org/dc/terms/coverage"/>
    </owl:AnnotationProperty>
    


    <!-- http://purl.org/dc/terms/title -->


    <rdf:Description rdf:about="http://purl.org/dc/terms/title">
        <rdfs:subPropertyOf rdf:resource="http://purl.org/dc/elements/1.1/title"/>
    </rdf:Description>
    


    <!-- http://purl.org/dc/terms/type -->


    <owl:AnnotationProperty rdf:about="http://purl.org/dc/terms/type">
        <rdfs:subPropertyOf rdf:resource="http://purl.org/dc/elements/1.1/type"/>
    </owl:AnnotationProperty>
    


    <!-- http://purl.org/dc/terms/valid -->


    <owl:AnnotationProperty rdf:about="http://purl.org/dc/terms/valid">
        <rdfs:subPropertyOf rdf:resource="http://purl.org/dc/elements/1.1/date"/>
    </owl:AnnotationProperty>
    


    <!-- http://purl.org/vocab/vann/example -->


    <owl:AnnotationProperty rdf:about="http://purl.org/vocab/vann/example"/>
    


    <!-- http://schema.org/#domainIncludes -->


    <owl:AnnotationProperty rdf:about="http://schema.org/#domainIncludes"/>
    


    <!-- 
    ///////////////////////////////////////////////////////////////////////////////////////
    //
    // Datatypes
    //
    ///////////////////////////////////////////////////////////////////////////////////////
     -->


    


    <!-- http://purl.org/dc/terms/Box -->


    <rdfs:Datatype rdf:about="http://purl.org/dc/terms/Box"/>
    


    <!-- http://purl.org/dc/terms/ISO3166 -->


    <rdfs:Datatype rdf:about="http://purl.org/dc/terms/ISO3166"/>
    


    <!-- http://purl.org/dc/terms/ISO639-2 -->


    <rdfs:Datatype rdf:about="http://purl.org/dc/terms/ISO639-2"/>
    


    <!-- http://purl.org/dc/terms/ISO639-3 -->


    <rdfs:Datatype rdf:about="http://purl.org/dc/terms/ISO639-3"/>
    


    <!-- http://purl.org/dc/terms/Period -->


    <rdfs:Datatype rdf:about="http://purl.org/dc/terms/Period"/>
    


    <!-- http://purl.org/dc/terms/Point -->


    <rdfs:Datatype rdf:about="http://purl.org/dc/terms/Point"/>
    


    <!-- http://purl.org/dc/terms/RFC1766 -->


    <rdfs:Datatype rdf:about="http://purl.org/dc/terms/RFC1766"/>
    


    <!-- http://purl.org/dc/terms/RFC3066 -->


    <rdfs:Datatype rdf:about="http://purl.org/dc/terms/RFC3066"/>
    


    <!-- http://purl.org/dc/terms/RFC4646 -->


    <rdfs:Datatype rdf:about="http://purl.org/dc/terms/RFC4646"/>
    


    <!-- http://purl.org/dc/terms/RFC5646 -->


    <rdfs:Datatype rdf:about="http://purl.org/dc/terms/RFC5646"/>
    


    <!-- http://purl.org/dc/terms/URI -->


    <rdfs:Datatype rdf:about="http://purl.org/dc/terms/URI"/>
    


    <!-- http://purl.org/dc/terms/W3CDTF -->


    <rdfs:Datatype rdf:about="http://purl.org/dc/terms/W3CDTF"/>
    


    <!-- http://www.w3.org/2001/XMLSchema#date -->


    <rdfs:Datatype rdf:about="http://www.w3.org/2001/XMLSchema#date"/>
    


    <!-- 
    ///////////////////////////////////////////////////////////////////////////////////////
    //
    // Object Properties
    //
    ///////////////////////////////////////////////////////////////////////////////////////
     -->


    


    <!-- http://webprotege.stanford.edu/RkSo6PclimyTVhUedJeJUk -->


    <owl:ObjectProperty rdf:about="http://webprotege.stanford.edu/RkSo6PclimyTVhUedJeJUk">
        <owl:inverseOf rdf:resource="urn:webprotege:ontology:dc88ba2e-7e28-4c89-8637-655a2b9ad945#belongsto"/>
        <rdfs:domain rdf:resource="https://pi.pauwel.be/voc/buildingelement#Roof"/>
        <rdfs:range rdf:resource="http://webprotege.stanford.edu/RCsOXjQhDvzdCqC92ncCBu"/>
        <rdfs:comment>Represents a part–whole relationship where a roof consists of one or more pitches.
Conceptually aligned with standard part–whole relations (e.g. BFO:has_part), without importing upper-level ontologies.</rdfs:comment>
        <rdfs:label>has Pitch</rdfs:label>
    </owl:ObjectProperty>
    


    <!-- https://w3id.org/dot#documentationFromInspection -->


    <owl:ObjectProperty rdf:about="https://w3id.org/dot#documentationFromInspection">
        <rdfs:domain rdf:resource="https://w3id.org/dot#Documentation"/>
        <rdfs:range rdf:resource="https://w3id.org/dot#Inspection"/>
    </owl:ObjectProperty>
    


    <!-- https://w3id.org/rdo#HasAppearance -->


    <owl:ObjectProperty rdf:about="https://w3id.org/rdo#HasAppearance">
        <owl:inverseOf rdf:resource="https://w3id.org/rdo#is_Inspection_Observation_Of"/>
        <rdfs:domain rdf:resource="https://w3id.org/dot#Damage"/>
        <rdfs:range rdf:resource="https://w3id.org/rdo#Damage_Inspection_Observation"/>
        <rdfs:comment>Relationship between a damage presence and the corresponding inspection observation.</rdfs:comment>
        <rdfs:label>has Inspection Observation</rdfs:label>
    </owl:ObjectProperty>
    


    <!-- https://w3id.org/rdo#Is_Composed_Of -->


    <owl:ObjectProperty rdf:about="https://w3id.org/rdo#Is_Composed_Of">
        <rdfs:domain rdf:resource="https://w3id.org/dot#Damage"/>
        <rdfs:range rdf:resource="https://w3id.org/dot#Damage"/>
        <rdfs:comment>Relationship between classified damage instances forming a composite classified damage.</rdfs:comment>
        <rdfs:label>is Composed Of</rdfs:label>
    </owl:ObjectProperty>
    


    <!-- https://w3id.org/rdo#affect_Product -->


    <owl:ObjectProperty rdf:about="https://w3id.org/rdo#affect_Product">
        <rdfs:domain rdf:resource="https://w3id.org/dot#Damage"/>
        <rdfs:range rdf:resource="https://schema.org/Product"/>
        <rdfs:comment>Relationship between a damage and the product it affects.</rdfs:comment>
        <rdfs:label>affects Product</rdfs:label>
    </owl:ObjectProperty>
    


    <!-- https://w3id.org/rdo#has_Damage_Observation_Location -->


    <owl:ObjectProperty rdf:about="https://w3id.org/rdo#has_Damage_Observation_Location">
        <owl:inverseOf rdf:resource="https://w3id.org/rdo#has_Image"/>
        <rdfs:domain rdf:resource="https://w3id.org/rdo#Image"/>
        <rdfs:range rdf:resource="https://w3id.org/rdo#Damage_Image_Location"/>
        <rdfs:comment>Relationship between an Image and one or more Damage Observation Image Locations recorded within that image.
This property is the inverse of has Image and enables queries from an image to the damage observation locations it contains.</rdfs:comment>
        <rdfs:label>has Damage Observation Location</rdfs:label>
    </owl:ObjectProperty>
    


    <!-- https://w3id.org/rdo#has_Image -->


    <owl:ObjectProperty rdf:about="https://w3id.org/rdo#has_Image">
        <rdfs:domain rdf:resource="https://w3id.org/rdo#Damage_Image_Location"/>
        <rdfs:range rdf:resource="https://w3id.org/rdo#Image"/>
        <rdfs:comment>Relationship between a damage image location and the corresponding image.</rdfs:comment>
        <rdfs:label>has Image</rdfs:label>
    </owl:ObjectProperty>
    


    <!-- https://w3id.org/rdo#has_Location_in -->


    <owl:ObjectProperty rdf:about="https://w3id.org/rdo#has_Location_in">
        <owl:inverseOf rdf:resource="https://w3id.org/rdo#locates_Damage"/>
        <rdfs:domain rdf:resource="https://w3id.org/rdo#Damage_Inspection_Observation"/>
        <rdfs:range rdf:resource="https://w3id.org/rdo#Damage_Image_Location"/>
        <rdfs:comment>Links a Damage Inspection Observation to the corresponding Damage Observation Image Location where it is spatially located within visual documentation.
This property is the inverse of locates and enables queries from inspection observations to their associated image locations.</rdfs:comment>
        <rdfs:label>has Location In</rdfs:label>
    </owl:ObjectProperty>
    


    <!-- https://w3id.org/rdo#is_Inspection_Observation_Of -->


    <owl:ObjectProperty rdf:about="https://w3id.org/rdo#is_Inspection_Observation_Of">
        <rdfs:comment>Relationship between an inspection observation and the corresponding damage entity</rdfs:comment>
        <rdfs:label>is Inspection Observation Of</rdfs:label>
    </owl:ObjectProperty>
    


    <!-- https://w3id.org/rdo#locates_Damage -->


    <owl:ObjectProperty rdf:about="https://w3id.org/rdo#locates_Damage">
        <rdfs:domain rdf:resource="https://w3id.org/rdo#Damage_Image_Location"/>
        <rdfs:range rdf:resource="https://w3id.org/rdo#Damage_Inspection_Observation"/>
        <rdfs:comment>Represents the relationship between a damage image location (e.g. a region on an orthophoto) and the damage inspection observation it refers to.
This allows a detected damage observed during an inspection to be spatially located within visual documentation.</rdfs:comment>
        <rdfs:label>locates</rdfs:label>
    </owl:ObjectProperty>
    


    <!-- urn:webprotege:ontology:dc88ba2e-7e28-4c89-8637-655a2b9ad945#belongsto -->


    <owl:ObjectProperty rdf:about="urn:webprotege:ontology:dc88ba2e-7e28-4c89-8637-655a2b9ad945#belongsto">
        <rdfs:domain rdf:resource="http://webprotege.stanford.edu/RCsOXjQhDvzdCqC92ncCBu"/>
        <rdfs:range rdf:resource="https://pi.pauwel.be/voc/buildingelement#Roof"/>
        <rdfs:comment>Relationship between a pitch and the roof it belongs to.</rdfs:comment>
        <rdfs:label>is Pitch Of</rdfs:label>
    </owl:ObjectProperty>
    


    <!-- 
    ///////////////////////////////////////////////////////////////////////////////////////
    //
    // Data properties
    //
    ///////////////////////////////////////////////////////////////////////////////////////
     -->


    


    <!-- http://purl.org/dc/terms/alternative -->


    <owl:DatatypeProperty rdf:about="http://purl.org/dc/terms/alternative">
        <rdfs:subPropertyOf rdf:resource="http://purl.org/dc/terms/title"/>
        <rdfs:range rdf:resource="http://www.w3.org/2000/01/rdf-schema#Literal"/>
    </owl:DatatypeProperty>
    


    <!-- http://purl.org/dc/terms/available -->


    <owl:DatatypeProperty rdf:about="http://purl.org/dc/terms/available">
        <rdfs:subPropertyOf rdf:resource="http://purl.org/dc/terms/date"/>
        <rdfs:range rdf:resource="http://www.w3.org/2000/01/rdf-schema#Literal"/>
    </owl:DatatypeProperty>
    


    <!-- http://purl.org/dc/terms/bibliographicCitation -->


    <owl:DatatypeProperty rdf:about="http://purl.org/dc/terms/bibliographicCitation">
        <rdfs:subPropertyOf rdf:resource="http://purl.org/dc/terms/identifier"/>
        <rdfs:range rdf:resource="http://www.w3.org/2000/01/rdf-schema#Literal"/>
    </owl:DatatypeProperty>
    


    <!-- http://purl.org/dc/terms/created -->


    <owl:DatatypeProperty rdf:about="http://purl.org/dc/terms/created">
        <rdfs:subPropertyOf rdf:resource="http://purl.org/dc/terms/date"/>
        <rdfs:range rdf:resource="http://www.w3.org/2000/01/rdf-schema#Literal"/>
    </owl:DatatypeProperty>
    


    <!-- http://purl.org/dc/terms/date -->


    <owl:DatatypeProperty rdf:about="http://purl.org/dc/terms/date">
        <rdfs:domain rdf:resource="https://w3id.org/dot#Inspection"/>
        <rdfs:range rdf:resource="http://www.w3.org/2000/01/rdf-schema#Literal"/>
    </owl:DatatypeProperty>
    


    <!-- http://purl.org/dc/terms/dateAccepted -->


    <owl:DatatypeProperty rdf:about="http://purl.org/dc/terms/dateAccepted">
        <rdfs:subPropertyOf rdf:resource="http://purl.org/dc/terms/date"/>
        <rdfs:range rdf:resource="http://www.w3.org/2000/01/rdf-schema#Literal"/>
    </owl:DatatypeProperty>
    


    <!-- http://purl.org/dc/terms/dateCopyrighted -->


    <owl:DatatypeProperty rdf:about="http://purl.org/dc/terms/dateCopyrighted">
        <rdfs:subPropertyOf rdf:resource="http://purl.org/dc/terms/date"/>
        <rdfs:range rdf:resource="http://www.w3.org/2000/01/rdf-schema#Literal"/>
    </owl:DatatypeProperty>
    


    <!-- http://purl.org/dc/terms/dateSubmitted -->


    <owl:DatatypeProperty rdf:about="http://purl.org/dc/terms/dateSubmitted">
        <rdfs:subPropertyOf rdf:resource="http://purl.org/dc/terms/date"/>
        <rdfs:range rdf:resource="http://www.w3.org/2000/01/rdf-schema#Literal"/>
    </owl:DatatypeProperty>
    


    <!-- http://purl.org/dc/terms/identifier -->


    <owl:DatatypeProperty rdf:about="http://purl.org/dc/terms/identifier">
        <rdfs:range rdf:resource="http://www.w3.org/2000/01/rdf-schema#Literal"/>
    </owl:DatatypeProperty>
    


    <!-- http://purl.org/dc/terms/issued -->


    <owl:DatatypeProperty rdf:about="http://purl.org/dc/terms/issued">
        <rdfs:subPropertyOf rdf:resource="http://purl.org/dc/terms/date"/>
        <rdfs:range rdf:resource="http://www.w3.org/2000/01/rdf-schema#Literal"/>
    </owl:DatatypeProperty>
    


    <!-- http://purl.org/dc/terms/modified -->


    <owl:DatatypeProperty rdf:about="http://purl.org/dc/terms/modified">
        <rdfs:subPropertyOf rdf:resource="http://purl.org/dc/terms/date"/>
        <rdfs:range rdf:resource="http://www.w3.org/2000/01/rdf-schema#Literal"/>
    </owl:DatatypeProperty>
    


    <!-- http://purl.org/dc/terms/title -->


    <owl:DatatypeProperty rdf:about="http://purl.org/dc/terms/title">
        <rdfs:range rdf:resource="http://www.w3.org/2000/01/rdf-schema#Literal"/>
    </owl:DatatypeProperty>
    


    <!-- http://purl.org/dc/terms/valid -->


    <owl:DatatypeProperty rdf:about="http://purl.org/dc/terms/valid">
        <rdfs:subPropertyOf rdf:resource="http://purl.org/dc/terms/date"/>
        <rdfs:range rdf:resource="http://www.w3.org/2000/01/rdf-schema#Literal"/>
    </owl:DatatypeProperty>
    


    <!-- http://webprotege.stanford.edu/RB3bxfNs0KGdXacZxMLhjzb -->


    <owl:DatatypeProperty rdf:about="http://webprotege.stanford.edu/RB3bxfNs0KGdXacZxMLhjzb">
        <rdfs:subPropertyOf rdf:resource="http://www.w3.org/2002/07/owl#topDataProperty"/>
        <rdfs:domain rdf:resource="https://w3id.org/dot#Damage"/>
        <rdfs:range rdf:resource="http://www.w3.org/2001/XMLSchema#decimal"/>
        <rdfs:comment>The confidence associated with an observation or assessment of a damage.</rdfs:comment>
        <rdfs:label>confidence</rdfs:label>
    </owl:DatatypeProperty>
    


    <!-- http://xmlns.com/foaf/0.1/name -->


    <rdf:Description rdf:about="http://xmlns.com/foaf/0.1/name">
        <rdfs:domain rdf:resource="http://xmlns.com/foaf/0.1/Person"/>
        <rdfs:range rdf:resource="http://www.w3.org/2001/XMLSchema#string"/>
    </rdf:Description>
    


    <!-- https://w3id.org/rdo#Caveat -->


    <owl:DatatypeProperty rdf:about="https://w3id.org/rdo#Caveat">
        <rdfs:domain rdf:resource="https://w3id.org/dot#Inspection"/>
        <rdfs:range rdf:resource="http://www.w3.org/2001/XMLSchema#string"/>
        <rdfs:comment>Specifies how inspection data were acquired, describing the data acquisition method used during an inspection (e.g. UAV-based photogrammetry, ground-based visual inspection, handheld photography, or mixed approaches). This property supports interpretation of inspection outcomes by making data provenance explicit.</rdfs:comment>
        <rdfs:label>data acquisition type</rdfs:label>
    </owl:DatatypeProperty>
    


    <!-- https://w3id.org/rdo#analysis_type -->


    <owl:DatatypeProperty rdf:about="https://w3id.org/rdo#analysis_type">
        <rdfs:domain rdf:resource="https://w3id.org/dot#Inspection"/>
        <rdfs:range rdf:resource="http://www.w3.org/2001/XMLSchema#string"/>
        <rdfs:comment>Specifies the type of analysis applied to inspection data, such as AI-assisted image analysis, manual expert assessment, or hybrid approaches. This property clarifies how inspection findings and defect classifications were produced, and helps to make potential limitations of the inspection results explicit.</rdfs:comment>
        <rdfs:label>analysis type</rdfs:label>
    </owl:DatatypeProperty>
    


    <!-- https://w3id.org/rdo#climate_context -->


    <owl:DatatypeProperty rdf:about="https://w3id.org/rdo#climate_context">
        <rdfs:subPropertyOf rdf:resource="https://w3id.org/rdo#environmental_and_climate_context"/>
        <rdfs:domain rdf:resource="https://schema.org/Product"/>
        <rdfs:range rdf:resource="http://www.w3.org/2001/XMLSchema#string"/>
        <rdfs:comment>Indicates the broader climatic setting relevant to the building (e.g., Scottish, English, inland, coastal), reflecting long-term exposure conditions such as rainfall patterns, wind-driven rain, freeze–thaw cycles, and humidity. Climate context supports comparison across inspections and helps explain differing deterioration rates observed on similar roof constructions.</rdfs:comment>
        <rdfs:label>climate context</rdfs:label>
    </owl:DatatypeProperty>
    


    <!-- https://w3id.org/rdo#environmental_and_climate_context -->


    <owl:DatatypeProperty rdf:about="https://w3id.org/rdo#environmental_and_climate_context">
        <rdfs:domain rdf:resource="https://w3id.org/dot#Damage"/>
        <rdfs:range rdf:resource="http://www.w3.org/2001/XMLSchema#string"/>
        <rdfs:comment>A grouping property for environmental and climatic context attributes that provide background conditions for roof inspection and condition assessment. These contextual properties do not describe individual defects or components directly, but support interpretation of observed deterioration patterns, moisture-related issues, and long-term weathering behaviour across the building.
This property is currently modelled as a simplified, free-text attribute and may be replaced in future work by links to dedicated weather and climate ontologies or external data sources (e.g. weather APIs and ontologies such as https://bimerr.iot.linkeddata.es/def/weather/), enabling more structured and time-specific representations.</rdfs:comment>
        <rdfs:label>environmental and climate context</rdfs:label>
    </owl:DatatypeProperty>
    


    <!-- https://w3id.org/rdo#environmental_context -->


    <owl:DatatypeProperty rdf:about="https://w3id.org/rdo#environmental_context">
        <rdfs:subPropertyOf rdf:resource="https://w3id.org/rdo#environmental_and_climate_context"/>
        <rdfs:domain rdf:resource="https://schema.org/Product"/>
        <rdfs:range rdf:resource="http://www.w3.org/2001/XMLSchema#string"/>
        <rdfs:comment>Describes the surrounding environmental setting of the building (e.g., urban, rural, coastal), representing site-level conditions shared by all roof elements. Environmental context helps inspectors interpret observed conditions, such as pollution-related soiling, vegetation growth, or persistent moisture, rather than serving as a direct indicator of defect presence.</rdfs:comment>
        <rdfs:label>environmental context</rdfs:label>
    </owl:DatatypeProperty>
    


    <!-- https://w3id.org/rdo#exposure_level -->


    <owl:DatatypeProperty rdf:about="https://w3id.org/rdo#exposure_level">
        <rdfs:subPropertyOf rdf:resource="https://w3id.org/rdo#environmental_and_climate_context"/>
        <rdfs:domain rdf:resource="http://webprotege.stanford.edu/RCsOXjQhDvzdCqC92ncCBu"/>
        <rdfs:range rdf:resource="http://www.w3.org/2001/XMLSchema#string"/>
        <rdfs:comment>Characterises the degree to which a pitch is exposed to weathering forces (e.g., sheltered or exposed). Exposure level influences the likelihood of wind-driven rain penetration, accelerated weathering of materials, and deterioration at junctions, but does not alone determine the presence or severity of defects.</rdfs:comment>
        <rdfs:label>exposure level</rdfs:label>
    </owl:DatatypeProperty>
    


    <!-- https://w3id.org/rdo#hasConditionLevel -->


    <owl:DatatypeProperty rdf:about="https://w3id.org/rdo#hasConditionLevel">
        <rdf:type rdf:resource="http://www.w3.org/2002/07/owl#FunctionalProperty"/>
        <rdfs:domain rdf:resource="https://schema.org/Product"/>
        <rdfs:range rdf:resource="http://www.w3.org/2001/XMLSchema#string"/>
        <rdfs:comment>Represents the assessed condition rating of a building element (e.g., roof or roof pitch), derived from visual inspection and used to indicate the severity of deterioration and the urgency of maintenance or repair. 
The value typically follows standardised building survey rating systems, such as the RICS Condition Ratings (1–3, traffic light system) or equivalent condition indices (e.g., numerical scales indicating maintenance, restoration, or replacement needs).</rdfs:comment>
        <rdfs:label>condition level</rdfs:label>
    </owl:DatatypeProperty>
    


    <!-- https://w3id.org/rdo#hasDefectType -->


    <owl:DatatypeProperty rdf:about="https://w3id.org/rdo#hasDefectType">
        <rdfs:domain rdf:resource="https://w3id.org/dot#ClassifiedDamage"/>
        <rdfs:range rdf:resource="http://www.w3.org/2001/XMLSchema#string"/>
        <rdfs:comment>This data property specifies the type of defect identified for a Classified Damage during roof inspection.

The defect types are expressed as descriptive values rather than modelled as individuals. They reflect inspection outcomes and expert interpretation.

Typical defect types include:

Slate Biological Growth (subclass of Classified Damage):
– algae: thin biological growth typically associated with surface moisture and damp environmental conditions;
– lichen: slow-growing biological organisms indicating long-term environmental exposure;
– moss: thicker biological growth that retains moisture and may contribute to accelerated material deterioration.

Slate Structural Defect (subclass of Classified Damage):
– broken slate: cracked or fractured slate that may allow water penetration;
– displaced slate: slate that has moved from its original position, potentially compromising weather tightness;
– missing slate: complete absence of a slate, directly exposing underlying roof layers.

The listed defect types are illustrative and not intended to form an exhaustive taxonomy.</rdfs:comment>
        <rdfs:label>Defect type</rdfs:label>
    </owl:DatatypeProperty>
    


    <!-- https://w3id.org/rdo#hasRepairStatus -->


    <owl:DatatypeProperty rdf:about="https://w3id.org/rdo#hasRepairStatus">
        <rdfs:domain rdf:resource="https://w3id.org/dot#ClassifiedDamage"/>
        <rdfs:range rdf:resource="http://www.w3.org/2001/XMLSchema#string"/>
        <rdfs:comment>Represents the observed or inferred repair status of a damage instance relative to the latest available inspection results, and where applicable, comparisons across multiple inspections.

The status reflects the current observation-based interpretation and does not necessarily indicate the existence of an explicit repair record.

Typical values include:

- &quot;active&quot;: The damage is explicitly detected and confirmed to be present in the latest inspection.
- &quot;not_observed&quot;: The damage is not detected in the latest inspection. This does not imply that the damage has been repaired, as the absence may be due to occlusion, limited visibility, data quality issues, or detection uncertainty.
- &quot;likely_repaired&quot;: Based on comparisons across multiple inspections, there is strong observational evidence suggesting that the damage may have been repaired; however, no explicit repair record or confirmation is available.
- &quot;confirmed_repaired&quot;: The damage is considered repaired based on explicit confirmation, such as a repair record, maintenance documentation, or expert validation. This status indicates recorded confirmation rather than purely observation-based inference.</rdfs:comment>
        <rdfs:label>repair status</rdfs:label>
    </owl:DatatypeProperty>
    


    <!-- https://w3id.org/rdo#hasResolution -->


    <owl:DatatypeProperty rdf:about="https://w3id.org/rdo#hasResolution">
        <rdfs:domain rdf:resource="https://w3id.org/rdo#Image"/>
        <rdfs:range rdf:resource="http://www.w3.org/2001/XMLSchema#decimal"/>
        <rdfs:comment>The resolution of the orthophoto, representing the size of each pixel in meters. For example, a value of &quot;0.005&quot; means each pixel represents 5mm by 5mm.</rdfs:comment>
        <rdfs:label>resolution</rdfs:label>
    </owl:DatatypeProperty>
    


    <!-- https://w3id.org/rdo#hasX -->


    <owl:DatatypeProperty rdf:about="https://w3id.org/rdo#hasX">
        <rdfs:domain rdf:resource="https://w3id.org/dot#Damage"/>
        <rdfs:comment>The XYZ coordinate of a damage instance, expressed in the same spatial reference system as the associated survey or orthophoto.</rdfs:comment>
        <rdfs:label>xyz</rdfs:label>
    </owl:DatatypeProperty>
    


    <!-- https://w3id.org/rdo#junction_context -->


    <owl:DatatypeProperty rdf:about="https://w3id.org/rdo#junction_context">
        <rdfs:domain rdf:resource="https://w3id.org/dot#Damage"/>
        <rdfs:range rdf:resource="http://www.w3.org/2001/XMLSchema#string"/>
        <rdfs:comment>A description of whether and how a damage is associated with a junction. This property is used to record junction-related context that is difficult to capture purely geometrically, such as “junction between slate and leadwork (material junction)” or “junction between roof and masonry (element junction)”. Junction information supports interpretation of likely failure mechanisms and potential water ingress pathways.</rdfs:comment>
        <rdfs:label>junction context</rdfs:label>
    </owl:DatatypeProperty>
    


    <!-- https://w3id.org/rdo#junction_type -->


    <owl:DatatypeProperty rdf:about="https://w3id.org/rdo#junction_type">
        <rdfs:subPropertyOf rdf:resource="http://www.w3.org/2002/07/owl#topDataProperty"/>
        <rdfs:domain rdf:resource="https://w3id.org/dot#Damage"/>
        <rdfs:range rdf:resource="http://www.w3.org/2001/XMLSchema#string"/>
        <rdfs:comment>Indicates the junction category relevant to the damage (e.g., material junction or element junction). This supports consistent reporting and querying of junction-related failures.</rdfs:comment>
        <rdfs:label>junction type</rdfs:label>
    </owl:DatatypeProperty>
    


    <!-- https://w3id.org/rdo#orientation -->


    <owl:DatatypeProperty rdf:about="https://w3id.org/rdo#orientation">
        <rdfs:subPropertyOf rdf:resource="https://w3id.org/rdo#environmental_and_climate_context"/>
        <rdfs:domain rdf:resource="http://webprotege.stanford.edu/RCsOXjQhDvzdCqC92ncCBu"/>
        <rdfs:range rdf:resource="http://www.w3.org/2001/XMLSchema#string"/>
        <rdfs:comment>Represents the facing direction (aspect) of a pitch (e.g., cardinal direction or azimuth). Orientation is pitch-specific and supports interpretation of differential moisture retention, biological growth, and weathering patterns observed during inspection, particularly where multiple pitches on the same roof exhibit different deterioration behaviours.</rdfs:comment>
        <rdfs:label>orientation</rdfs:label>
    </owl:DatatypeProperty>
    


    <!-- https://w3id.org/rdo#pitch_angle -->


    <owl:DatatypeProperty rdf:about="https://w3id.org/rdo#pitch_angle">
        <rdfs:domain rdf:resource="http://webprotege.stanford.edu/RCsOXjQhDvzdCqC92ncCBu"/>
        <rdfs:range rdf:resource="http://www.w3.org/2001/XMLSchema#decimal"/>
        <rdfs:comment>Pitch angle is a numerical value (expressed in degrees) representing the inclination of a roof surface. This property uses a decimal value to allow precise measurement. Indicative threshold ranges may be applied for roof characterisation: pitch angles below 10° typically indicate flat roofs; values between 10° and 45° represent low-pitched roofs; and angles greater than 45° indicate steeply pitched roofs. Variations in pitch angle influence drainage behaviour, exposure conditions, defect susceptibility, and inspection and maintenance considerations.</rdfs:comment>
        <rdfs:label>Pitch angle</rdfs:label>
    </owl:DatatypeProperty>
    


    <!-- https://w3id.org/rdo#relative_position -->


    <owl:DatatypeProperty rdf:about="https://w3id.org/rdo#relative_position">
        <rdfs:subPropertyOf rdf:resource="https://w3id.org/rdo#environmental_and_climate_context"/>
        <rdfs:domain rdf:resource="http://webprotege.stanford.edu/RCsOXjQhDvzdCqC92ncCBu"/>
        <rdfs:range rdf:resource="http://www.w3.org/2001/XMLSchema#string"/>
        <rdfs:comment>Specifies the relative position of a pitch within the overall roof configuration (e.g., upper pitch or lower pitch). Relative position is important for inspection interpretation, as lower pitches may receive runoff, debris, or moisture from higher pitches, and are often associated with junction-related issues and concealed water ingress pathways.</rdfs:comment>
        <rdfs:label>relative position</rdfs:label>
    </owl:DatatypeProperty>
    


    <!-- https://w3id.org/rdo#roof_build_up -->


    <owl:DatatypeProperty rdf:about="https://w3id.org/rdo#roof_build_up">
        <rdfs:subPropertyOf rdf:resource="http://www.w3.org/2002/07/owl#topDataProperty"/>
        <rdfs:domain rdf:resource="https://pi.pauwel.be/voc/buildingelement#Roof"/>
        <rdfs:range rdf:resource="http://www.w3.org/2001/XMLSchema#string"/>
        <rdfs:comment>A description of the roof build-up (construction make-up), capturing the main roof-related elements and underlying materials relevant to condition assessment. This may include slates, ridge coverings, mortar fillets at wall abutments, lead flashings, wallhead/parapet gutters, chimney stacks, associated stonework/brickwork, and underlying layers such as masonry, lead, mortar, sarking/timber, or flat-roofing materials. This property is intended to record practical construction knowledge often missing from BIM models and to support interpretation of junction-related defects and water ingress mechanisms.</rdfs:comment>
        <rdfs:label>Roof build-up</rdfs:label>
    </owl:DatatypeProperty>
    


    <!-- 
    ///////////////////////////////////////////////////////////////////////////////////////
    //
    // Classes
    //
    ///////////////////////////////////////////////////////////////////////////////////////
     -->


    


    <!-- http://purl.org/dc/dcam/VocabularyEncodingScheme -->


    <owl:Class rdf:about="http://purl.org/dc/dcam/VocabularyEncodingScheme"/>
    


    <!-- http://purl.org/dc/terms/Agent -->


    <owl:Class rdf:about="http://purl.org/dc/terms/Agent"/>
    


    <!-- http://purl.org/dc/terms/AgentClass -->


    <owl:Class rdf:about="http://purl.org/dc/terms/AgentClass">
        <rdfs:subClassOf rdf:resource="http://www.w3.org/2000/01/rdf-schema#Class"/>
    </owl:Class>
    


    <!-- http://purl.org/dc/terms/BibliographicResource -->


    <owl:Class rdf:about="http://purl.org/dc/terms/BibliographicResource"/>
    


    <!-- http://purl.org/dc/terms/FileFormat -->


    <owl:Class rdf:about="http://purl.org/dc/terms/FileFormat">
        <rdfs:subClassOf rdf:resource="http://purl.org/dc/terms/MediaType"/>
    </owl:Class>
    


    <!-- http://purl.org/dc/terms/Frequency -->


    <owl:Class rdf:about="http://purl.org/dc/terms/Frequency"/>
    


    <!-- http://purl.org/dc/terms/Jurisdiction -->


    <owl:Class rdf:about="http://purl.org/dc/terms/Jurisdiction">
        <rdfs:subClassOf rdf:resource="http://purl.org/dc/terms/LocationPeriodOrJurisdiction"/>
    </owl:Class>
    


    <!-- http://purl.org/dc/terms/LicenseDocument -->


    <owl:Class rdf:about="http://purl.org/dc/terms/LicenseDocument">
        <rdfs:subClassOf rdf:resource="http://purl.org/dc/terms/RightsStatement"/>
    </owl:Class>
    


    <!-- http://purl.org/dc/terms/LinguisticSystem -->


    <owl:Class rdf:about="http://purl.org/dc/terms/LinguisticSystem"/>
    


    <!-- http://purl.org/dc/terms/Location -->


    <owl:Class rdf:about="http://purl.org/dc/terms/Location">
        <rdfs:subClassOf rdf:resource="http://purl.org/dc/terms/LocationPeriodOrJurisdiction"/>
    </owl:Class>
    


    <!-- http://purl.org/dc/terms/LocationPeriodOrJurisdiction -->


    <owl:Class rdf:about="http://purl.org/dc/terms/LocationPeriodOrJurisdiction"/>
    


    <!-- http://purl.org/dc/terms/MediaType -->


    <owl:Class rdf:about="http://purl.org/dc/terms/MediaType">
        <rdfs:subClassOf rdf:resource="http://purl.org/dc/terms/MediaTypeOrExtent"/>
    </owl:Class>
    


    <!-- http://purl.org/dc/terms/MediaTypeOrExtent -->


    <owl:Class rdf:about="http://purl.org/dc/terms/MediaTypeOrExtent"/>
    


    <!-- http://purl.org/dc/terms/MethodOfAccrual -->


    <owl:Class rdf:about="http://purl.org/dc/terms/MethodOfAccrual"/>
    


    <!-- http://purl.org/dc/terms/MethodOfInstruction -->


    <owl:Class rdf:about="http://purl.org/dc/terms/MethodOfInstruction"/>
    


    <!-- http://purl.org/dc/terms/PeriodOfTime -->


    <owl:Class rdf:about="http://purl.org/dc/terms/PeriodOfTime">
        <rdfs:subClassOf rdf:resource="http://purl.org/dc/terms/LocationPeriodOrJurisdiction"/>
    </owl:Class>
    


    <!-- http://purl.org/dc/terms/PhysicalMedium -->


    <owl:Class rdf:about="http://purl.org/dc/terms/PhysicalMedium">
        <rdfs:subClassOf rdf:resource="http://purl.org/dc/terms/MediaType"/>
    </owl:Class>
    


    <!-- http://purl.org/dc/terms/PhysicalResource -->


    <owl:Class rdf:about="http://purl.org/dc/terms/PhysicalResource"/>
    


    <!-- http://purl.org/dc/terms/Policy -->


    <owl:Class rdf:about="http://purl.org/dc/terms/Policy"/>
    


    <!-- http://purl.org/dc/terms/ProvenanceStatement -->


    <owl:Class rdf:about="http://purl.org/dc/terms/ProvenanceStatement"/>
    


    <!-- http://purl.org/dc/terms/RightsStatement -->


    <owl:Class rdf:about="http://purl.org/dc/terms/RightsStatement"/>
    


    <!-- http://purl.org/dc/terms/SizeOrDuration -->


    <owl:Class rdf:about="http://purl.org/dc/terms/SizeOrDuration">
        <rdfs:subClassOf rdf:resource="http://purl.org/dc/terms/MediaTypeOrExtent"/>
    </owl:Class>
    


    <!-- http://purl.org/dc/terms/Standard -->


    <owl:Class rdf:about="http://purl.org/dc/terms/Standard"/>
    


    <!-- http://webprotege.stanford.edu/R89LStemoQ1MqtJ4u3wNnCc -->


    <owl:Class rdf:about="http://webprotege.stanford.edu/R89LStemoQ1MqtJ4u3wNnCc">
        <rdfs:subClassOf rdf:resource="https://w3id.org/dot#ClassifiedDamage"/>
        <rdfs:comment>A Slate Structural Defect represents a physical damage potentially affecting the integrity or position of a roof slate, such as broken, displaced, or missing slate.</rdfs:comment>
        <rdfs:label>Slate Structural Defect</rdfs:label>
    </owl:Class>
    


    <!-- http://webprotege.stanford.edu/RCY2aGVeb8KpRCsVrf5s8AD -->


    <owl:Class rdf:about="http://webprotege.stanford.edu/RCY2aGVeb8KpRCsVrf5s8AD">
        <rdfs:subClassOf rdf:resource="https://w3id.org/rdo#Image"/>
        <rdfs:comment>An Orthophoto is a geometrically corrected image produced from photogrammetric processing, providing a uniform scale representation of roof surfaces and serving as spatial evidence for damage documentation.</rdfs:comment>
        <rdfs:label>Orthophoto</rdfs:label>
    </owl:Class>
    


    <!-- http://webprotege.stanford.edu/RCiwm3pFp97sUUNZMKSqwg7 -->


    <owl:Class rdf:about="http://webprotege.stanford.edu/RCiwm3pFp97sUUNZMKSqwg7">
        <rdfs:subClassOf rdf:resource="https://w3id.org/dot#Inspection"/>
        <rdfs:comment>A Roof Inspection is a specialised inspection activity focusing on the condition assessment of roof elements, during which visual observations, images, and damage documentation are produced</rdfs:comment>
        <rdfs:label>Roof Inspection</rdfs:label>
    </owl:Class>
    


    <!-- http://webprotege.stanford.edu/RCsOXjQhDvzdCqC92ncCBu -->


    <owl:Class rdf:about="http://webprotege.stanford.edu/RCsOXjQhDvzdCqC92ncCBu">
        <rdfs:subClassOf rdf:resource="https://pi.pauwel.be/voc/buildingelement#BuildingElementPart"/>
        <rdfs:comment>A Roof Pitch is a subdivision of a roof used as a spatial unit for inspection and damage documentation.</rdfs:comment>
        <rdfs:label>Roof Pitch</rdfs:label>
    </owl:Class>
    


    <!-- http://webprotege.stanford.edu/RkC6OzV1rmYsTeyuPAyaTf -->


    <owl:Class rdf:about="http://webprotege.stanford.edu/RkC6OzV1rmYsTeyuPAyaTf">
        <rdfs:subClassOf rdf:resource="https://w3id.org/dot#ClassifiedDamage"/>
        <rdfs:comment>Slate Biological Growth represents biologically induced surface conditions observed on roof slates, such as algae, moss, and lichen. These forms of growth are not necessarily defects in themselves, but are indicative of persistent moisture, local environmental conditions, and reduced drying potential. The presence and distribution of biological growth may signal emerging risks, particularly at junctions or areas prone to water retention, and therefore support interpretation of roof condition and prioritisation of further inspection.</rdfs:comment>
        <rdfs:label>Slate Biological Growth</rdfs:label>
    </owl:Class>
    


    <!-- http://www.w3.org/2000/01/rdf-schema#Class -->


    <owl:Class rdf:about="http://www.w3.org/2000/01/rdf-schema#Class"/>
    


    <!-- http://xmlns.com/foaf/0.1/Image -->


    <owl:Class rdf:about="http://xmlns.com/foaf/0.1/Image">
        <owl:equivalentClass rdf:resource="https://w3id.org/rdo#Image"/>
    </owl:Class>
    


    <!-- https://w3id.org/dot#ClassifiedDamage -->


    <owl:Class rdf:about="https://w3id.org/dot#ClassifiedDamage"/>
    


    <!-- https://w3id.org/dot#Damage -->


    <owl:Class rdf:about="https://w3id.org/dot#Damage"/>
    


    <!-- https://w3id.org/dot#Documentation -->


    <owl:Class rdf:about="https://w3id.org/dot#Documentation"/>
    


    <!-- https://w3id.org/dot#ExternalResource -->


    <owl:Class rdf:about="https://w3id.org/dot#ExternalResource"/>
    


    <!-- https://w3id.org/dot#Inspection -->


    <owl:Class rdf:about="https://w3id.org/dot#Inspection"/>
    


    <!-- https://w3id.org/rdo#Damage_Image_Location -->


    <owl:Class rdf:about="https://w3id.org/rdo#Damage_Image_Location">
        <rdfs:comment>A Damage Observation Image Location represents the spatial localisation of a detected or observed damage within an image or orthophoto.</rdfs:comment>
        <rdfs:label>Damage Observation Image Location</rdfs:label>
    </owl:Class>
    


    <!-- https://w3id.org/rdo#Damage_Inspection_Observation -->


    <owl:Class rdf:about="https://w3id.org/rdo#Damage_Inspection_Observation">
        <rdfs:subClassOf rdf:resource="https://w3id.org/dot#Damage"/>
        <rdfs:comment>A Damage Inspection Observation represents an observation made during an inspection indicating the presence of a potential damage.</rdfs:comment>
        <rdfs:label>Damage Inspection Observation</rdfs:label>
    </owl:Class>
    


    <!-- https://w3id.org/rdo#Image -->


    <owl:Class rdf:about="https://w3id.org/rdo#Image">
        <rdfs:subClassOf rdf:resource="https://w3id.org/dot#ExternalResource"/>
    </owl:Class>
    


    <!-- 
    ///////////////////////////////////////////////////////////////////////////////////////
    //
    // Individuals
    //
    ///////////////////////////////////////////////////////////////////////////////////////
     -->


    


    <!-- http://purl.org/dc/terms/ -->


    <owl:NamedIndividual rdf:about="http://purl.org/dc/terms/">
        <terms:modified rdf:datatype="http://www.w3.org/2001/XMLSchema#date">2012-06-14</terms:modified>
        <terms:title xml:lang="en">DCMI Metadata Terms - other</terms:title>
        <terms:publisher rdf:resource="http://purl.org/dc/aboutdcmi#DCMI"/>
    </owl:NamedIndividual>
    


    <!-- http://purl.org/dc/terms/Agent -->


    <owl:NamedIndividual rdf:about="http://purl.org/dc/terms/Agent">
        <rdf:type rdf:resource="http://purl.org/dc/terms/AgentClass"/>
        <terms:issued rdf:datatype="http://www.w3.org/2001/XMLSchema#date">2008-01-14</terms:issued>
    </owl:NamedIndividual>
    


    <!-- http://purl.org/dc/terms/AgentClass -->


    <owl:NamedIndividual rdf:about="http://purl.org/dc/terms/AgentClass">
        <terms:issued rdf:datatype="http://www.w3.org/2001/XMLSchema#date">2008-01-14</terms:issued>
    </owl:NamedIndividual>
    


    <!-- http://purl.org/dc/terms/BibliographicResource -->


    <owl:NamedIndividual rdf:about="http://purl.org/dc/terms/BibliographicResource">
        <terms:issued rdf:datatype="http://www.w3.org/2001/XMLSchema#date">2008-01-14</terms:issued>
    </owl:NamedIndividual>
    


    <!-- http://purl.org/dc/terms/Box -->


    <owl:NamedIndividual rdf:about="http://purl.org/dc/terms/Box">
        <terms:issued rdf:datatype="http://www.w3.org/2001/XMLSchema#date">2000-07-11</terms:issued>
    </owl:NamedIndividual>
    


    <!-- http://purl.org/dc/terms/DCMIType -->


    <owl:NamedIndividual rdf:about="http://purl.org/dc/terms/DCMIType">
        <rdf:type rdf:resource="http://purl.org/dc/dcam/VocabularyEncodingScheme"/>
        <terms:issued rdf:datatype="http://www.w3.org/2001/XMLSchema#date">2000-07-11</terms:issued>
        <rdfs:comment xml:lang="en">The set of classes specified by the DCMI Type Vocabulary, used to categorize the nature or genre of the resource.</rdfs:comment>
        <rdfs:isDefinedBy rdf:resource="http://purl.org/dc/terms/"/>
        <rdfs:label xml:lang="en">DCMI Type Vocabulary</rdfs:label>
        <rdfs:seeAlso rdf:resource="http://purl.org/dc/dcmitype/"/>
    </owl:NamedIndividual>
    


    <!-- http://purl.org/dc/terms/DDC -->


    <owl:NamedIndividual rdf:about="http://purl.org/dc/terms/DDC">
        <rdf:type rdf:resource="http://purl.org/dc/dcam/VocabularyEncodingScheme"/>
        <terms:issued rdf:datatype="http://www.w3.org/2001/XMLSchema#date">2000-07-11</terms:issued>
        <rdfs:comment xml:lang="en">The set of conceptual resources specified by the Dewey Decimal Classification.</rdfs:comment>
        <rdfs:isDefinedBy rdf:resource="http://purl.org/dc/terms/"/>
        <rdfs:label xml:lang="en">DDC</rdfs:label>
        <rdfs:seeAlso rdf:resource="http://www.oclc.org/dewey/"/>
    </owl:NamedIndividual>
    


    <!-- http://purl.org/dc/terms/FileFormat -->


    <owl:NamedIndividual rdf:about="http://purl.org/dc/terms/FileFormat">
        <terms:issued rdf:datatype="http://www.w3.org/2001/XMLSchema#date">2008-01-14</terms:issued>
    </owl:NamedIndividual>
    


    <!-- http://purl.org/dc/terms/Frequency -->


    <owl:NamedIndividual rdf:about="http://purl.org/dc/terms/Frequency">
        <terms:issued rdf:datatype="http://www.w3.org/2001/XMLSchema#date">2008-01-14</terms:issued>
    </owl:NamedIndividual>
    


    <!-- http://purl.org/dc/terms/IMT -->


    <owl:NamedIndividual rdf:about="http://purl.org/dc/terms/IMT">
        <rdf:type rdf:resource="http://purl.org/dc/dcam/VocabularyEncodingScheme"/>
        <terms:issued rdf:datatype="http://www.w3.org/2001/XMLSchema#date">2000-07-11</terms:issued>
        <rdfs:comment xml:lang="en">The set of media types specified by the Internet Assigned Numbers Authority.</rdfs:comment>
        <rdfs:isDefinedBy rdf:resource="http://purl.org/dc/terms/"/>
        <rdfs:label xml:lang="en">IMT</rdfs:label>
        <rdfs:seeAlso rdf:resource="http://www.iana.org/assignments/media-types/"/>
    </owl:NamedIndividual>
    


    <!-- http://purl.org/dc/terms/ISO3166 -->


    <owl:NamedIndividual rdf:about="http://purl.org/dc/terms/ISO3166">
        <terms:issued rdf:datatype="http://www.w3.org/2001/XMLSchema#date">2000-07-11</terms:issued>
    </owl:NamedIndividual>
    


    <!-- http://purl.org/dc/terms/ISO639-2 -->


    <owl:NamedIndividual rdf:about="http://purl.org/dc/terms/ISO639-2">
        <terms:issued rdf:datatype="http://www.w3.org/2001/XMLSchema#date">2000-07-11</terms:issued>
    </owl:NamedIndividual>
    


    <!-- http://purl.org/dc/terms/ISO639-3 -->


    <owl:NamedIndividual rdf:about="http://purl.org/dc/terms/ISO639-3">
        <terms:issued rdf:datatype="http://www.w3.org/2001/XMLSchema#date">2008-01-14</terms:issued>
    </owl:NamedIndividual>
    


    <!-- http://purl.org/dc/terms/Jurisdiction -->


    <owl:NamedIndividual rdf:about="http://purl.org/dc/terms/Jurisdiction">
        <terms:issued rdf:datatype="http://www.w3.org/2001/XMLSchema#date">2008-01-14</terms:issued>
    </owl:NamedIndividual>
    


    <!-- http://purl.org/dc/terms/LCC -->


    <owl:NamedIndividual rdf:about="http://purl.org/dc/terms/LCC">
        <rdf:type rdf:resource="http://purl.org/dc/dcam/VocabularyEncodingScheme"/>
        <terms:issued rdf:datatype="http://www.w3.org/2001/XMLSchema#date">2000-07-11</terms:issued>
        <rdfs:comment xml:lang="en">The set of conceptual resources specified by the Library of Congress Classification.</rdfs:comment>
        <rdfs:isDefinedBy rdf:resource="http://purl.org/dc/terms/"/>
        <rdfs:label xml:lang="en">LCC</rdfs:label>
        <rdfs:seeAlso rdf:resource="http://lcweb.loc.gov/catdir/cpso/lcco/lcco.html"/>
    </owl:NamedIndividual>
    


    <!-- http://purl.org/dc/terms/LCSH -->


    <owl:NamedIndividual rdf:about="http://purl.org/dc/terms/LCSH">
        <rdf:type rdf:resource="http://purl.org/dc/dcam/VocabularyEncodingScheme"/>
        <terms:issued rdf:datatype="http://www.w3.org/2001/XMLSchema#date">2000-07-11</terms:issued>
        <rdfs:comment xml:lang="en">The set of labeled concepts specified by the Library of Congress Subject Headings.</rdfs:comment>
        <rdfs:isDefinedBy rdf:resource="http://purl.org/dc/terms/"/>
        <rdfs:label xml:lang="en">LCSH</rdfs:label>
    </owl:NamedIndividual>
    


    <!-- http://purl.org/dc/terms/LicenseDocument -->


    <owl:NamedIndividual rdf:about="http://purl.org/dc/terms/LicenseDocument">
        <terms:issued rdf:datatype="http://www.w3.org/2001/XMLSchema#date">2008-01-14</terms:issued>
    </owl:NamedIndividual>
    


    <!-- http://purl.org/dc/terms/LinguisticSystem -->


    <owl:NamedIndividual rdf:about="http://purl.org/dc/terms/LinguisticSystem">
        <terms:issued rdf:datatype="http://www.w3.org/2001/XMLSchema#date">2008-01-14</terms:issued>
    </owl:NamedIndividual>
    


    <!-- http://purl.org/dc/terms/Location -->


    <owl:NamedIndividual rdf:about="http://purl.org/dc/terms/Location">
        <terms:issued rdf:datatype="http://www.w3.org/2001/XMLSchema#date">2008-01-14</terms:issued>
    </owl:NamedIndividual>
    


    <!-- http://purl.org/dc/terms/LocationPeriodOrJurisdiction -->


    <owl:NamedIndividual rdf:about="http://purl.org/dc/terms/LocationPeriodOrJurisdiction">
        <terms:issued rdf:datatype="http://www.w3.org/2001/XMLSchema#date">2008-01-14</terms:issued>
    </owl:NamedIndividual>
    


    <!-- http://purl.org/dc/terms/MESH -->


    <owl:NamedIndividual rdf:about="http://purl.org/dc/terms/MESH">
        <rdf:type rdf:resource="http://purl.org/dc/dcam/VocabularyEncodingScheme"/>
        <terms:issued rdf:datatype="http://www.w3.org/2001/XMLSchema#date">2000-07-11</terms:issued>
        <rdfs:comment xml:lang="en">The set of labeled concepts specified by the Medical Subject Headings.</rdfs:comment>
        <rdfs:isDefinedBy rdf:resource="http://purl.org/dc/terms/"/>
        <rdfs:label xml:lang="en">MeSH</rdfs:label>
        <rdfs:seeAlso rdf:resource="http://www.nlm.nih.gov/mesh/meshhome.html"/>
    </owl:NamedIndividual>
    


    <!-- http://purl.org/dc/terms/MediaType -->


    <owl:NamedIndividual rdf:about="http://purl.org/dc/terms/MediaType">
        <terms:issued rdf:datatype="http://www.w3.org/2001/XMLSchema#date">2008-01-14</terms:issued>
    </owl:NamedIndividual>
    


    <!-- http://purl.org/dc/terms/MediaTypeOrExtent -->


    <owl:NamedIndividual rdf:about="http://purl.org/dc/terms/MediaTypeOrExtent">
        <terms:issued rdf:datatype="http://www.w3.org/2001/XMLSchema#date">2008-01-14</terms:issued>
    </owl:NamedIndividual>
    


    <!-- http://purl.org/dc/terms/MethodOfAccrual -->


    <owl:NamedIndividual rdf:about="http://purl.org/dc/terms/MethodOfAccrual">
        <terms:issued rdf:datatype="http://www.w3.org/2001/XMLSchema#date">2008-01-14</terms:issued>
    </owl:NamedIndividual>
    


    <!-- http://purl.org/dc/terms/MethodOfInstruction -->


    <owl:NamedIndividual rdf:about="http://purl.org/dc/terms/MethodOfInstruction">
        <terms:issued rdf:datatype="http://www.w3.org/2001/XMLSchema#date">2008-01-14</terms:issued>
    </owl:NamedIndividual>
    


    <!-- http://purl.org/dc/terms/NLM -->


    <owl:NamedIndividual rdf:about="http://purl.org/dc/terms/NLM">
        <rdf:type rdf:resource="http://purl.org/dc/dcam/VocabularyEncodingScheme"/>
        <terms:issued rdf:datatype="http://www.w3.org/2001/XMLSchema#date">2005-06-13</terms:issued>
        <rdfs:comment xml:lang="en">The set of conceptual resources specified by the National Library of Medicine Classification.</rdfs:comment>
        <rdfs:isDefinedBy rdf:resource="http://purl.org/dc/terms/"/>
        <rdfs:label xml:lang="en">NLM</rdfs:label>
        <rdfs:seeAlso rdf:resource="http://wwwcf.nlm.nih.gov/class/"/>
    </owl:NamedIndividual>
    


    <!-- http://purl.org/dc/terms/Period -->


    <owl:NamedIndividual rdf:about="http://purl.org/dc/terms/Period">
        <terms:issued rdf:datatype="http://www.w3.org/2001/XMLSchema#date">2000-07-11</terms:issued>
    </owl:NamedIndividual>
    


    <!-- http://purl.org/dc/terms/PeriodOfTime -->


    <owl:NamedIndividual rdf:about="http://purl.org/dc/terms/PeriodOfTime">
        <terms:issued rdf:datatype="http://www.w3.org/2001/XMLSchema#date">2008-01-14</terms:issued>
    </owl:NamedIndividual>
    


    <!-- http://purl.org/dc/terms/PhysicalMedium -->


    <owl:NamedIndividual rdf:about="http://purl.org/dc/terms/PhysicalMedium">
        <terms:issued rdf:datatype="http://www.w3.org/2001/XMLSchema#date">2008-01-14</terms:issued>
    </owl:NamedIndividual>
    


    <!-- http://purl.org/dc/terms/PhysicalResource -->


    <owl:NamedIndividual rdf:about="http://purl.org/dc/terms/PhysicalResource">
        <terms:issued rdf:datatype="http://www.w3.org/2001/XMLSchema#date">2008-01-14</terms:issued>
    </owl:NamedIndividual>
    


    <!-- http://purl.org/dc/terms/Point -->


    <owl:NamedIndividual rdf:about="http://purl.org/dc/terms/Point">
        <terms:issued rdf:datatype="http://www.w3.org/2001/XMLSchema#date">2000-07-11</terms:issued>
    </owl:NamedIndividual>
    


    <!-- http://purl.org/dc/terms/Policy -->


    <owl:NamedIndividual rdf:about="http://purl.org/dc/terms/Policy">
        <terms:issued rdf:datatype="http://www.w3.org/2001/XMLSchema#date">2008-01-14</terms:issued>
    </owl:NamedIndividual>
    


    <!-- http://purl.org/dc/terms/ProvenanceStatement -->


    <owl:NamedIndividual rdf:about="http://purl.org/dc/terms/ProvenanceStatement">
        <terms:issued rdf:datatype="http://www.w3.org/2001/XMLSchema#date">2008-01-14</terms:issued>
    </owl:NamedIndividual>
    


    <!-- http://purl.org/dc/terms/RFC1766 -->


    <owl:NamedIndividual rdf:about="http://purl.org/dc/terms/RFC1766">
        <terms:issued rdf:datatype="http://www.w3.org/2001/XMLSchema#date">2000-07-11</terms:issued>
    </owl:NamedIndividual>
    


    <!-- http://purl.org/dc/terms/RFC3066 -->


    <owl:NamedIndividual rdf:about="http://purl.org/dc/terms/RFC3066">
        <terms:issued rdf:datatype="http://www.w3.org/2001/XMLSchema#date">2002-07-13</terms:issued>
    </owl:NamedIndividual>
    


    <!-- http://purl.org/dc/terms/RFC4646 -->


    <owl:NamedIndividual rdf:about="http://purl.org/dc/terms/RFC4646">
        <terms:issued rdf:datatype="http://www.w3.org/2001/XMLSchema#date">2008-01-14</terms:issued>
    </owl:NamedIndividual>
    


    <!-- http://purl.org/dc/terms/RFC5646 -->


    <owl:NamedIndividual rdf:about="http://purl.org/dc/terms/RFC5646">
        <terms:issued rdf:datatype="http://www.w3.org/2001/XMLSchema#date">2010-10-11</terms:issued>
    </owl:NamedIndividual>
    


    <!-- http://purl.org/dc/terms/RightsStatement -->


    <owl:NamedIndividual rdf:about="http://purl.org/dc/terms/RightsStatement">
        <terms:issued rdf:datatype="http://www.w3.org/2001/XMLSchema#date">2008-01-14</terms:issued>
    </owl:NamedIndividual>
    


    <!-- http://purl.org/dc/terms/SizeOrDuration -->


    <owl:NamedIndividual rdf:about="http://purl.org/dc/terms/SizeOrDuration">
        <terms:issued rdf:datatype="http://www.w3.org/2001/XMLSchema#date">2008-01-14</terms:issued>
    </owl:NamedIndividual>
    


    <!-- http://purl.org/dc/terms/Standard -->


    <owl:NamedIndividual rdf:about="http://purl.org/dc/terms/Standard">
        <terms:issued rdf:datatype="http://www.w3.org/2001/XMLSchema#date">2008-01-14</terms:issued>
    </owl:NamedIndividual>
    


    <!-- http://purl.org/dc/terms/TGN -->


    <owl:NamedIndividual rdf:about="http://purl.org/dc/terms/TGN">
        <rdf:type rdf:resource="http://purl.org/dc/dcam/VocabularyEncodingScheme"/>
        <terms:issued rdf:datatype="http://www.w3.org/2001/XMLSchema#date">2000-07-11</terms:issued>
        <rdfs:comment xml:lang="en">The set of places specified by the Getty Thesaurus of Geographic Names.</rdfs:comment>
        <rdfs:isDefinedBy rdf:resource="http://purl.org/dc/terms/"/>
        <rdfs:label xml:lang="en">TGN</rdfs:label>
        <rdfs:seeAlso rdf:resource="http://www.getty.edu/research/tools/vocabulary/tgn/index.html"/>
    </owl:NamedIndividual>
    


    <!-- http://purl.org/dc/terms/UDC -->


    <owl:NamedIndividual rdf:about="http://purl.org/dc/terms/UDC">
        <rdf:type rdf:resource="http://purl.org/dc/dcam/VocabularyEncodingScheme"/>
        <terms:issued rdf:datatype="http://www.w3.org/2001/XMLSchema#date">2000-07-11</terms:issued>
        <rdfs:comment xml:lang="en">The set of conceptual resources specified by the Universal Decimal Classification.</rdfs:comment>
        <rdfs:isDefinedBy rdf:resource="http://purl.org/dc/terms/"/>
        <rdfs:label xml:lang="en">UDC</rdfs:label>
        <rdfs:seeAlso rdf:resource="http://www.udcc.org/"/>
    </owl:NamedIndividual>
    


    <!-- http://purl.org/dc/terms/URI -->


    <owl:NamedIndividual rdf:about="http://purl.org/dc/terms/URI">
        <terms:issued rdf:datatype="http://www.w3.org/2001/XMLSchema#date">2000-07-11</terms:issued>
    </owl:NamedIndividual>
    


    <!-- http://purl.org/dc/terms/W3CDTF -->


    <owl:NamedIndividual rdf:about="http://purl.org/dc/terms/W3CDTF">
        <terms:issued rdf:datatype="http://www.w3.org/2001/XMLSchema#date">2000-07-11</terms:issued>
    </owl:NamedIndividual>
    


    <!-- http://purl.org/dc/terms/abstract -->


    <owl:NamedIndividual rdf:about="http://purl.org/dc/terms/abstract">
        <terms:issued rdf:datatype="http://www.w3.org/2001/XMLSchema#date">2000-07-11</terms:issued>
    </owl:NamedIndividual>
    


    <!-- http://purl.org/dc/terms/accessRights -->


    <owl:NamedIndividual rdf:about="http://purl.org/dc/terms/accessRights">
        <terms:issued rdf:datatype="http://www.w3.org/2001/XMLSchema#date">2003-02-15</terms:issued>
    </owl:NamedIndividual>
    


    <!-- http://purl.org/dc/terms/accrualMethod -->


    <owl:NamedIndividual rdf:about="http://purl.org/dc/terms/accrualMethod">
        <terms:issued rdf:datatype="http://www.w3.org/2001/XMLSchema#date">2005-06-13</terms:issued>
    </owl:NamedIndividual>
    


    <!-- http://purl.org/dc/terms/accrualPeriodicity -->


    <owl:NamedIndividual rdf:about="http://purl.org/dc/terms/accrualPeriodicity">
        <terms:issued rdf:datatype="http://www.w3.org/2001/XMLSchema#date">2005-06-13</terms:issued>
    </owl:NamedIndividual>
    


    <!-- http://purl.org/dc/terms/accrualPolicy -->


    <owl:NamedIndividual rdf:about="http://purl.org/dc/terms/accrualPolicy">
        <terms:issued rdf:datatype="http://www.w3.org/2001/XMLSchema#date">2005-06-13</terms:issued>
    </owl:NamedIndividual>
    


    <!-- http://purl.org/dc/terms/alternative -->


    <owl:NamedIndividual rdf:about="http://purl.org/dc/terms/alternative">
        <terms:issued rdf:datatype="http://www.w3.org/2001/XMLSchema#date">2000-07-11</terms:issued>
    </owl:NamedIndividual>
    


    <!-- http://purl.org/dc/terms/audience -->


    <owl:NamedIndividual rdf:about="http://purl.org/dc/terms/audience">
        <terms:issued rdf:datatype="http://www.w3.org/2001/XMLSchema#date">2001-05-21</terms:issued>
    </owl:NamedIndividual>
    


    <!-- http://purl.org/dc/terms/available -->


    <owl:NamedIndividual rdf:about="http://purl.org/dc/terms/available">
        <terms:issued rdf:datatype="http://www.w3.org/2001/XMLSchema#date">2000-07-11</terms:issued>
    </owl:NamedIndividual>
    


    <!-- http://purl.org/dc/terms/bibliographicCitation -->


    <owl:NamedIndividual rdf:about="http://purl.org/dc/terms/bibliographicCitation">
        <terms:issued rdf:datatype="http://www.w3.org/2001/XMLSchema#date">2003-02-15</terms:issued>
    </owl:NamedIndividual>
    


    <!-- http://purl.org/dc/terms/conformsTo -->


    <owl:NamedIndividual rdf:about="http://purl.org/dc/terms/conformsTo">
        <terms:issued rdf:datatype="http://www.w3.org/2001/XMLSchema#date">2001-05-21</terms:issued>
    </owl:NamedIndividual>
    


    <!-- http://purl.org/dc/terms/contributor -->


    <owl:NamedIndividual rdf:about="http://purl.org/dc/terms/contributor">
        <terms:issued rdf:datatype="http://www.w3.org/2001/XMLSchema#date">2008-01-14</terms:issued>
    </owl:NamedIndividual>
    


    <!-- http://purl.org/dc/terms/coverage -->


    <owl:NamedIndividual rdf:about="http://purl.org/dc/terms/coverage">
        <terms:issued rdf:datatype="http://www.w3.org/2001/XMLSchema#date">2008-01-14</terms:issued>
    </owl:NamedIndividual>
    


    <!-- http://purl.org/dc/terms/created -->


    <owl:NamedIndividual rdf:about="http://purl.org/dc/terms/created">
        <terms:issued rdf:datatype="http://www.w3.org/2001/XMLSchema#date">2000-07-11</terms:issued>
    </owl:NamedIndividual>
    


    <!-- http://purl.org/dc/terms/creator -->


    <owl:NamedIndividual rdf:about="http://purl.org/dc/terms/creator">
        <terms:issued rdf:datatype="http://www.w3.org/2001/XMLSchema#date">2008-01-14</terms:issued>
    </owl:NamedIndividual>
    


    <!-- http://purl.org/dc/terms/date -->


    <owl:NamedIndividual rdf:about="http://purl.org/dc/terms/date">
        <terms:issued rdf:datatype="http://www.w3.org/2001/XMLSchema#date">2008-01-14</terms:issued>
    </owl:NamedIndividual>
    


    <!-- http://purl.org/dc/terms/dateAccepted -->


    <owl:NamedIndividual rdf:about="http://purl.org/dc/terms/dateAccepted">
        <terms:issued rdf:datatype="http://www.w3.org/2001/XMLSchema#date">2002-07-13</terms:issued>
    </owl:NamedIndividual>
    


    <!-- http://purl.org/dc/terms/dateCopyrighted -->


    <owl:NamedIndividual rdf:about="http://purl.org/dc/terms/dateCopyrighted">
        <terms:issued rdf:datatype="http://www.w3.org/2001/XMLSchema#date">2002-07-13</terms:issued>
    </owl:NamedIndividual>
    


    <!-- http://purl.org/dc/terms/dateSubmitted -->


    <owl:NamedIndividual rdf:about="http://purl.org/dc/terms/dateSubmitted">
        <terms:issued rdf:datatype="http://www.w3.org/2001/XMLSchema#date">2002-07-13</terms:issued>
    </owl:NamedIndividual>
    


    <!-- http://purl.org/dc/terms/description -->


    <owl:NamedIndividual rdf:about="http://purl.org/dc/terms/description">
        <terms:issued rdf:datatype="http://www.w3.org/2001/XMLSchema#date">2008-01-14</terms:issued>
    </owl:NamedIndividual>
    


    <!-- http://purl.org/dc/terms/educationLevel -->


    <owl:NamedIndividual rdf:about="http://purl.org/dc/terms/educationLevel">
        <terms:issued rdf:datatype="http://www.w3.org/2001/XMLSchema#date">2002-07-13</terms:issued>
    </owl:NamedIndividual>
    


    <!-- http://purl.org/dc/terms/extent -->


    <owl:NamedIndividual rdf:about="http://purl.org/dc/terms/extent">
        <terms:issued rdf:datatype="http://www.w3.org/2001/XMLSchema#date">2000-07-11</terms:issued>
    </owl:NamedIndividual>
    


    <!-- http://purl.org/dc/terms/format -->


    <owl:NamedIndividual rdf:about="http://purl.org/dc/terms/format">
        <terms:issued rdf:datatype="http://www.w3.org/2001/XMLSchema#date">2008-01-14</terms:issued>
    </owl:NamedIndividual>
    


    <!-- http://purl.org/dc/terms/hasFormat -->


    <owl:NamedIndividual rdf:about="http://purl.org/dc/terms/hasFormat">
        <terms:issued rdf:datatype="http://www.w3.org/2001/XMLSchema#date">2000-07-11</terms:issued>
    </owl:NamedIndividual>
    


    <!-- http://purl.org/dc/terms/hasPart -->


    <owl:NamedIndividual rdf:about="http://purl.org/dc/terms/hasPart">
        <terms:issued rdf:datatype="http://www.w3.org/2001/XMLSchema#date">2000-07-11</terms:issued>
    </owl:NamedIndividual>
    


    <!-- http://purl.org/dc/terms/hasVersion -->


    <owl:NamedIndividual rdf:about="http://purl.org/dc/terms/hasVersion">
        <terms:issued rdf:datatype="http://www.w3.org/2001/XMLSchema#date">2000-07-11</terms:issued>
    </owl:NamedIndividual>
    


    <!-- http://purl.org/dc/terms/identifier -->


    <owl:NamedIndividual rdf:about="http://purl.org/dc/terms/identifier">
        <terms:issued rdf:datatype="http://www.w3.org/2001/XMLSchema#date">2008-01-14</terms:issued>
    </owl:NamedIndividual>
    


    <!-- http://purl.org/dc/terms/instructionalMethod -->


    <owl:NamedIndividual rdf:about="http://purl.org/dc/terms/instructionalMethod">
        <terms:issued rdf:datatype="http://www.w3.org/2001/XMLSchema#date">2005-06-13</terms:issued>
        <dcam:rangeIncludes rdf:resource="http://purl.org/dc/terms/MethodOfInstruction"/>
        <terms:description xml:lang="en">Instructional Method typically includes ways of presenting instructional materials or conducting instructional activities, patterns of learner-to-learner and learner-to-instructor interactions, and mechanisms by which group and individual levels of learning are measured.  Instructional methods include all aspects of the instruction and learning processes from planning and implementation through evaluation and feedback.</terms:description>
        <rdfs:comment xml:lang="en">A process, used to engender knowledge, attitudes and skills, that the described resource is designed to support.</rdfs:comment>
        <rdfs:isDefinedBy rdf:resource="http://purl.org/dc/terms/"/>
        <rdfs:label xml:lang="en">Instructional Method</rdfs:label>
    </owl:NamedIndividual>
    


    <!-- http://purl.org/dc/terms/isFormatOf -->


    <owl:NamedIndividual rdf:about="http://purl.org/dc/terms/isFormatOf">
        <terms:issued rdf:datatype="http://www.w3.org/2001/XMLSchema#date">2000-07-11</terms:issued>
    </owl:NamedIndividual>
    


    <!-- http://purl.org/dc/terms/isPartOf -->


    <owl:NamedIndividual rdf:about="http://purl.org/dc/terms/isPartOf">
        <terms:issued rdf:datatype="http://www.w3.org/2001/XMLSchema#date">2000-07-11</terms:issued>
    </owl:NamedIndividual>
    


    <!-- http://purl.org/dc/terms/isReferencedBy -->


    <owl:NamedIndividual rdf:about="http://purl.org/dc/terms/isReferencedBy">
        <terms:issued rdf:datatype="http://www.w3.org/2001/XMLSchema#date">2000-07-11</terms:issued>
    </owl:NamedIndividual>
    


    <!-- http://purl.org/dc/terms/isReplacedBy -->


    <owl:NamedIndividual rdf:about="http://purl.org/dc/terms/isReplacedBy">
        <terms:issued rdf:datatype="http://www.w3.org/2001/XMLSchema#date">2000-07-11</terms:issued>
    </owl:NamedIndividual>
    


    <!-- http://purl.org/dc/terms/isRequiredBy -->


    <owl:NamedIndividual rdf:about="http://purl.org/dc/terms/isRequiredBy">
        <terms:issued rdf:datatype="http://www.w3.org/2001/XMLSchema#date">2000-07-11</terms:issued>
    </owl:NamedIndividual>
    


    <!-- http://purl.org/dc/terms/isVersionOf -->


    <owl:NamedIndividual rdf:about="http://purl.org/dc/terms/isVersionOf">
        <terms:issued rdf:datatype="http://www.w3.org/2001/XMLSchema#date">2000-07-11</terms:issued>
    </owl:NamedIndividual>
    


    <!-- http://purl.org/dc/terms/issued -->


    <owl:DatatypeProperty rdf:about="http://purl.org/dc/terms/issued">
        <rdf:type rdf:resource="http://www.w3.org/2002/07/owl#NamedIndividual"/>
        <terms:issued rdf:datatype="http://www.w3.org/2001/XMLSchema#date">2000-07-11</terms:issued>
    </owl:DatatypeProperty>
    


    <!-- http://purl.org/dc/terms/language -->


    <owl:NamedIndividual rdf:about="http://purl.org/dc/terms/language">
        <terms:issued rdf:datatype="http://www.w3.org/2001/XMLSchema#date">2008-01-14</terms:issued>
    </owl:NamedIndividual>
    


    <!-- http://purl.org/dc/terms/license -->


    <owl:NamedIndividual rdf:about="http://purl.org/dc/terms/license">
        <terms:issued rdf:datatype="http://www.w3.org/2001/XMLSchema#date">2004-06-14</terms:issued>
    </owl:NamedIndividual>
    


    <!-- http://purl.org/dc/terms/mediator -->


    <owl:NamedIndividual rdf:about="http://purl.org/dc/terms/mediator">
        <terms:issued rdf:datatype="http://www.w3.org/2001/XMLSchema#date">2001-05-21</terms:issued>
    </owl:NamedIndividual>
    


    <!-- http://purl.org/dc/terms/medium -->


    <owl:NamedIndividual rdf:about="http://purl.org/dc/terms/medium">
        <terms:issued rdf:datatype="http://www.w3.org/2001/XMLSchema#date">2000-07-11</terms:issued>
    </owl:NamedIndividual>
    


    <!-- http://purl.org/dc/terms/modified -->


    <owl:NamedIndividual rdf:about="http://purl.org/dc/terms/modified">
        <terms:issued rdf:datatype="http://www.w3.org/2001/XMLSchema#date">2000-07-11</terms:issued>
    </owl:NamedIndividual>
    


    <!-- http://purl.org/dc/terms/provenance -->


    <owl:NamedIndividual rdf:about="http://purl.org/dc/terms/provenance">
        <terms:issued rdf:datatype="http://www.w3.org/2001/XMLSchema#date">2004-09-20</terms:issued>
        <dcam:rangeIncludes rdf:resource="http://purl.org/dc/terms/ProvenanceStatement"/>
        <terms:description xml:lang="en">The statement may include a description of any changes successive custodians made to the resource.</terms:description>
        <rdfs:comment xml:lang="en">A statement of any changes in ownership and custody of the resource since its creation that are significant for its authenticity, integrity, and interpretation.</rdfs:comment>
        <rdfs:isDefinedBy rdf:resource="http://purl.org/dc/terms/"/>
        <rdfs:label xml:lang="en">Provenance</rdfs:label>
    </owl:NamedIndividual>
    


    <!-- http://purl.org/dc/terms/publisher -->


    <owl:NamedIndividual rdf:about="http://purl.org/dc/terms/publisher">
        <terms:issued rdf:datatype="http://www.w3.org/2001/XMLSchema#date">2008-01-14</terms:issued>
    </owl:NamedIndividual>
    


    <!-- http://purl.org/dc/terms/references -->


    <owl:NamedIndividual rdf:about="http://purl.org/dc/terms/references">
        <terms:issued rdf:datatype="http://www.w3.org/2001/XMLSchema#date">2000-07-11</terms:issued>
    </owl:NamedIndividual>
    


    <!-- http://purl.org/dc/terms/relation -->


    <owl:NamedIndividual rdf:about="http://purl.org/dc/terms/relation">
        <terms:issued rdf:datatype="http://www.w3.org/2001/XMLSchema#date">2008-01-14</terms:issued>
    </owl:NamedIndividual>
    


    <!-- http://purl.org/dc/terms/replaces -->


    <owl:NamedIndividual rdf:about="http://purl.org/dc/terms/replaces">
        <terms:issued rdf:datatype="http://www.w3.org/2001/XMLSchema#date">2000-07-11</terms:issued>
    </owl:NamedIndividual>
    


    <!-- http://purl.org/dc/terms/requires -->


    <owl:NamedIndividual rdf:about="http://purl.org/dc/terms/requires">
        <terms:issued rdf:datatype="http://www.w3.org/2001/XMLSchema#date">2000-07-11</terms:issued>
    </owl:NamedIndividual>
    


    <!-- http://purl.org/dc/terms/rights -->


    <owl:NamedIndividual rdf:about="http://purl.org/dc/terms/rights">
        <terms:issued rdf:datatype="http://www.w3.org/2001/XMLSchema#date">2008-01-14</terms:issued>
    </owl:NamedIndividual>
    


    <!-- http://purl.org/dc/terms/rightsHolder -->


    <owl:NamedIndividual rdf:about="http://purl.org/dc/terms/rightsHolder">
        <terms:issued rdf:datatype="http://www.w3.org/2001/XMLSchema#date">2004-06-14</terms:issued>
        <dcam:rangeIncludes rdf:resource="http://purl.org/dc/terms/Agent"/>
        <terms:description xml:lang="en">Recommended practice is to refer to the rights holder with a URI. If this is not possible or feasible, a literal value that identifies the rights holder may be provided.</terms:description>
        <rdfs:comment xml:lang="en">A person or organization owning or managing rights over the resource.</rdfs:comment>
        <rdfs:isDefinedBy rdf:resource="http://purl.org/dc/terms/"/>
        <rdfs:label xml:lang="en">Rights Holder</rdfs:label>
    </owl:NamedIndividual>
    


    <!-- http://purl.org/dc/terms/source -->


    <owl:NamedIndividual rdf:about="http://purl.org/dc/terms/source">
        <terms:issued rdf:datatype="http://www.w3.org/2001/XMLSchema#date">2008-01-14</terms:issued>
    </owl:NamedIndividual>
    


    <!-- http://purl.org/dc/terms/spatial -->


    <owl:NamedIndividual rdf:about="http://purl.org/dc/terms/spatial">
        <terms:issued rdf:datatype="http://www.w3.org/2001/XMLSchema#date">2000-07-11</terms:issued>
    </owl:NamedIndividual>
    


    <!-- http://purl.org/dc/terms/subject -->


    <owl:NamedIndividual rdf:about="http://purl.org/dc/terms/subject">
        <terms:issued rdf:datatype="http://www.w3.org/2001/XMLSchema#date">2008-01-14</terms:issued>
    </owl:NamedIndividual>
    


    <!-- http://purl.org/dc/terms/tableOfContents -->


    <owl:NamedIndividual rdf:about="http://purl.org/dc/terms/tableOfContents">
        <terms:issued rdf:datatype="http://www.w3.org/2001/XMLSchema#date">2000-07-11</terms:issued>
    </owl:NamedIndividual>
    


    <!-- http://purl.org/dc/terms/temporal -->


    <owl:NamedIndividual rdf:about="http://purl.org/dc/terms/temporal">
        <terms:issued rdf:datatype="http://www.w3.org/2001/XMLSchema#date">2000-07-11</terms:issued>
    </owl:NamedIndividual>
    


    <!-- http://purl.org/dc/terms/title -->


    <owl:NamedIndividual rdf:about="http://purl.org/dc/terms/title">
        <terms:issued rdf:datatype="http://www.w3.org/2001/XMLSchema#date">2008-01-14</terms:issued>
    </owl:NamedIndividual>
    


    <!-- http://purl.org/dc/terms/type -->


    <owl:NamedIndividual rdf:about="http://purl.org/dc/terms/type">
        <terms:issued rdf:datatype="http://www.w3.org/2001/XMLSchema#date">2008-01-14</terms:issued>
    </owl:NamedIndividual>
    


    <!-- http://purl.org/dc/terms/valid -->


    <owl:NamedIndividual rdf:about="http://purl.org/dc/terms/valid">
        <terms:issued rdf:datatype="http://www.w3.org/2001/XMLSchema#date">2000-07-11</terms:issued>
    </owl:NamedIndividual>
    


    <!-- 
    ///////////////////////////////////////////////////////////////////////////////////////
    //
    // Annotations
    //
    ///////////////////////////////////////////////////////////////////////////////////////
     -->


    <rdf:Description rdf:about="http://purl.org/dc/terms/Agent">
        <rdfs:comment xml:lang="en">A resource that acts or has the power to act.</rdfs:comment>
        <rdfs:isDefinedBy rdf:resource="http://purl.org/dc/terms/"/>
        <rdfs:label xml:lang="en">Agent</rdfs:label>
    </rdf:Description>
    <rdf:Description rdf:about="http://purl.org/dc/terms/AgentClass">
        <rdfs:comment xml:lang="en">A group of agents.</rdfs:comment>
        <rdfs:isDefinedBy rdf:resource="http://purl.org/dc/terms/"/>
        <rdfs:label xml:lang="en">Agent Class</rdfs:label>
    </rdf:Description>
    <rdf:Description rdf:about="http://purl.org/dc/terms/BibliographicResource">
        <rdfs:comment xml:lang="en">A book, article, or other documentary resource.</rdfs:comment>
        <rdfs:isDefinedBy rdf:resource="http://purl.org/dc/terms/"/>
        <rdfs:label xml:lang="en">Bibliographic Resource</rdfs:label>
    </rdf:Description>
    <rdf:Description rdf:about="http://purl.org/dc/terms/Box">
        <rdfs:comment xml:lang="en">The set of regions in space defined by their geographic coordinates according to the DCMI Box Encoding Scheme.</rdfs:comment>
        <rdfs:isDefinedBy rdf:resource="http://purl.org/dc/terms/"/>
        <rdfs:label xml:lang="en">DCMI Box</rdfs:label>
        <rdfs:seeAlso rdf:resource="https://www.dublincore.org/specifications/dublin-core/dcmi-box/"/>
    </rdf:Description>
    <rdf:Description rdf:about="http://purl.org/dc/terms/FileFormat">
        <rdfs:comment xml:lang="en">A digital resource format.</rdfs:comment>
        <rdfs:isDefinedBy rdf:resource="http://purl.org/dc/terms/"/>
        <rdfs:label xml:lang="en">File Format</rdfs:label>
    </rdf:Description>
    <rdf:Description rdf:about="http://purl.org/dc/terms/Frequency">
        <rdfs:comment xml:lang="en">A rate at which something recurs.</rdfs:comment>
        <rdfs:isDefinedBy rdf:resource="http://purl.org/dc/terms/"/>
        <rdfs:label xml:lang="en">Frequency</rdfs:label>
    </rdf:Description>
    <rdf:Description rdf:about="http://purl.org/dc/terms/ISO3166">
        <rdfs:comment xml:lang="en">The set of codes listed in ISO 3166-1 for the representation of names of countries.</rdfs:comment>
        <rdfs:isDefinedBy rdf:resource="http://purl.org/dc/terms/"/>
        <rdfs:label xml:lang="en">ISO 3166</rdfs:label>
        <rdfs:seeAlso rdf:resource="https://www.iso.org/obp/ui/#search"/>
    </rdf:Description>
    <rdf:Description rdf:about="http://purl.org/dc/terms/ISO639-2">
        <rdfs:comment xml:lang="en">The three-letter alphabetic codes listed in ISO639-2 for the representation of names of languages.</rdfs:comment>
        <rdfs:isDefinedBy rdf:resource="http://purl.org/dc/terms/"/>
        <rdfs:label xml:lang="en">ISO 639-2</rdfs:label>
        <rdfs:seeAlso rdf:resource="http://lcweb.loc.gov/standards/iso639-2/langhome.html"/>
    </rdf:Description>
    <rdf:Description rdf:about="http://purl.org/dc/terms/ISO639-3">
        <rdfs:comment xml:lang="en">The set of three-letter codes listed in ISO 639-3 for the representation of names of languages.</rdfs:comment>
        <rdfs:isDefinedBy rdf:resource="http://purl.org/dc/terms/"/>
        <rdfs:label xml:lang="en">ISO 639-3</rdfs:label>
        <rdfs:seeAlso rdf:resource="http://www.sil.org/iso639-3/"/>
    </rdf:Description>
    <rdf:Description rdf:about="http://purl.org/dc/terms/Jurisdiction">
        <rdfs:comment xml:lang="en">The extent or range of judicial, law enforcement, or other authority.</rdfs:comment>
        <rdfs:isDefinedBy rdf:resource="http://purl.org/dc/terms/"/>
        <rdfs:label xml:lang="en">Jurisdiction</rdfs:label>
    </rdf:Description>
    <rdf:Description rdf:about="http://purl.org/dc/terms/LicenseDocument">
        <rdfs:comment xml:lang="en">A legal document giving official permission to do something with a resource.</rdfs:comment>
        <rdfs:isDefinedBy rdf:resource="http://purl.org/dc/terms/"/>
        <rdfs:label xml:lang="en">License Document</rdfs:label>
    </rdf:Description>
    <rdf:Description rdf:about="http://purl.org/dc/terms/LinguisticSystem">
        <terms:description xml:lang="en">Written, spoken, sign, and computer languages are linguistic systems.</terms:description>
        <rdfs:comment xml:lang="en">A system of signs, symbols, sounds, gestures, or rules used in communication.</rdfs:comment>
        <rdfs:isDefinedBy rdf:resource="http://purl.org/dc/terms/"/>
        <rdfs:label xml:lang="en">Linguistic System</rdfs:label>
    </rdf:Description>
    <rdf:Description rdf:about="http://purl.org/dc/terms/Location">
        <rdfs:comment xml:lang="en">A spatial region or named place.</rdfs:comment>
        <rdfs:isDefinedBy rdf:resource="http://purl.org/dc/terms/"/>
        <rdfs:label xml:lang="en">Location</rdfs:label>
    </rdf:Description>
    <rdf:Description rdf:about="http://purl.org/dc/terms/LocationPeriodOrJurisdiction">
        <rdfs:comment xml:lang="en">A location, period of time, or jurisdiction.</rdfs:comment>
        <rdfs:isDefinedBy rdf:resource="http://purl.org/dc/terms/"/>
        <rdfs:label xml:lang="en">Location, Period, or Jurisdiction</rdfs:label>
    </rdf:Description>
    <rdf:Description rdf:about="http://purl.org/dc/terms/MediaType">
        <rdfs:comment xml:lang="en">A file format or physical medium.</rdfs:comment>
        <rdfs:isDefinedBy rdf:resource="http://purl.org/dc/terms/"/>
        <rdfs:label xml:lang="en">Media Type</rdfs:label>
    </rdf:Description>
    <rdf:Description rdf:about="http://purl.org/dc/terms/MediaTypeOrExtent">
        <rdfs:comment xml:lang="en">A media type or extent.</rdfs:comment>
        <rdfs:isDefinedBy rdf:resource="http://purl.org/dc/terms/"/>
        <rdfs:label xml:lang="en">Media Type or Extent</rdfs:label>
    </rdf:Description>
    <rdf:Description rdf:about="http://purl.org/dc/terms/MethodOfAccrual">
        <rdfs:comment xml:lang="en">A method by which resources are added to a collection.</rdfs:comment>
        <rdfs:isDefinedBy rdf:resource="http://purl.org/dc/terms/"/>
        <rdfs:label xml:lang="en">Method of Accrual</rdfs:label>
    </rdf:Description>
    <rdf:Description rdf:about="http://purl.org/dc/terms/MethodOfInstruction">
        <rdfs:comment xml:lang="en">A process that is used to engender knowledge, attitudes, and skills.</rdfs:comment>
        <rdfs:isDefinedBy rdf:resource="http://purl.org/dc/terms/"/>
        <rdfs:label xml:lang="en">Method of Instruction</rdfs:label>
    </rdf:Description>
    <rdf:Description rdf:about="http://purl.org/dc/terms/Period">
        <rdfs:comment xml:lang="en">The set of time intervals defined by their limits according to the DCMI Period Encoding Scheme.</rdfs:comment>
        <rdfs:isDefinedBy rdf:resource="http://purl.org/dc/terms/"/>
        <rdfs:label xml:lang="en">DCMI Period</rdfs:label>
        <rdfs:seeAlso rdf:resource="https://www.dublincore.org/specifications/dublin-core/dcmi-period/"/>
    </rdf:Description>
    <rdf:Description rdf:about="http://purl.org/dc/terms/PeriodOfTime">
        <rdfs:comment xml:lang="en">An interval of time that is named or defined by its start and end dates.</rdfs:comment>
        <rdfs:isDefinedBy rdf:resource="http://purl.org/dc/terms/"/>
        <rdfs:label xml:lang="en">Period of Time</rdfs:label>
    </rdf:Description>
    <rdf:Description rdf:about="http://purl.org/dc/terms/PhysicalMedium">
        <terms:description xml:lang="en">Examples include paper, canvas, or DVD.</terms:description>
        <rdfs:comment xml:lang="en">A physical material or carrier.</rdfs:comment>
        <rdfs:isDefinedBy rdf:resource="http://purl.org/dc/terms/"/>
        <rdfs:label xml:lang="en">Physical Medium</rdfs:label>
    </rdf:Description>
    <rdf:Description rdf:about="http://purl.org/dc/terms/PhysicalResource">
        <rdfs:comment xml:lang="en">A material thing.</rdfs:comment>
        <rdfs:isDefinedBy rdf:resource="http://purl.org/dc/terms/"/>
        <rdfs:label xml:lang="en">Physical Resource</rdfs:label>
    </rdf:Description>
    <rdf:Description rdf:about="http://purl.org/dc/terms/Point">
        <rdfs:comment xml:lang="en">The set of points in space defined by their geographic coordinates according to the DCMI Point Encoding Scheme.</rdfs:comment>
        <rdfs:isDefinedBy rdf:resource="http://purl.org/dc/terms/"/>
        <rdfs:label xml:lang="en">DCMI Point</rdfs:label>
        <rdfs:seeAlso rdf:resource="https://www.dublincore.org/specifications/dublin-core/dcmi-point/"/>
    </rdf:Description>
    <rdf:Description rdf:about="http://purl.org/dc/terms/Policy">
        <rdfs:comment xml:lang="en">A plan or course of action by an authority, intended to influence and determine decisions, actions, and other matters.</rdfs:comment>
        <rdfs:isDefinedBy rdf:resource="http://purl.org/dc/terms/"/>
        <rdfs:label xml:lang="en">Policy</rdfs:label>
    </rdf:Description>
    <rdf:Description rdf:about="http://purl.org/dc/terms/ProvenanceStatement">
        <rdfs:comment xml:lang="en">Any changes in ownership and custody of a resource since its creation that are significant for its authenticity, integrity, and interpretation.</rdfs:comment>
        <rdfs:isDefinedBy rdf:resource="http://purl.org/dc/terms/"/>
        <rdfs:label xml:lang="en">Provenance Statement</rdfs:label>
    </rdf:Description>
    <rdf:Description rdf:about="http://purl.org/dc/terms/RFC1766">
        <rdfs:comment xml:lang="en">The set of tags, constructed according to RFC 1766, for the identification of languages.</rdfs:comment>
        <rdfs:isDefinedBy rdf:resource="http://purl.org/dc/terms/"/>
        <rdfs:label xml:lang="en">RFC 1766</rdfs:label>
        <rdfs:seeAlso rdf:resource="http://www.ietf.org/rfc/rfc1766.txt"/>
    </rdf:Description>
    <rdf:Description rdf:about="http://purl.org/dc/terms/RFC3066">
        <terms:description xml:lang="en">RFC 3066 has been obsoleted by RFC 4646.</terms:description>
        <rdfs:comment xml:lang="en">The set of tags constructed according to RFC 3066 for the identification of languages.</rdfs:comment>
        <rdfs:isDefinedBy rdf:resource="http://purl.org/dc/terms/"/>
        <rdfs:label xml:lang="en">RFC 3066</rdfs:label>
        <rdfs:seeAlso rdf:resource="http://www.ietf.org/rfc/rfc3066.txt"/>
    </rdf:Description>
    <rdf:Description rdf:about="http://purl.org/dc/terms/RFC4646">
        <terms:description xml:lang="en">RFC 4646 obsoletes RFC 3066.</terms:description>
        <rdfs:comment xml:lang="en">The set of tags constructed according to RFC 4646 for the identification of languages.</rdfs:comment>
        <rdfs:isDefinedBy rdf:resource="http://purl.org/dc/terms/"/>
        <rdfs:label xml:lang="en">RFC 4646</rdfs:label>
        <rdfs:seeAlso rdf:resource="http://www.ietf.org/rfc/rfc4646.txt"/>
    </rdf:Description>
    <rdf:Description rdf:about="http://purl.org/dc/terms/RFC5646">
        <terms:description xml:lang="en">RFC 5646 obsoletes RFC 4646.</terms:description>
        <rdfs:comment xml:lang="en">The set of tags constructed according to RFC 5646 for the identification of languages.</rdfs:comment>
        <rdfs:isDefinedBy rdf:resource="http://purl.org/dc/terms/"/>
        <rdfs:label xml:lang="en">RFC 5646</rdfs:label>
        <rdfs:seeAlso rdf:resource="http://www.ietf.org/rfc/rfc5646.txt"/>
    </rdf:Description>
    <rdf:Description rdf:about="http://purl.org/dc/terms/RightsStatement">
        <rdfs:comment xml:lang="en">A statement about the intellectual property rights (IPR) held in or over a resource, a legal document giving official permission to do something with a resource, or a statement about access rights.</rdfs:comment>
        <rdfs:isDefinedBy rdf:resource="http://purl.org/dc/terms/"/>
        <rdfs:label xml:lang="en">Rights Statement</rdfs:label>
    </rdf:Description>
    <rdf:Description rdf:about="http://purl.org/dc/terms/SizeOrDuration">
        <terms:description xml:lang="en">Examples include a number of pages, a specification of length, width, and breadth, or a period in hours, minutes, and seconds.</terms:description>
        <rdfs:comment xml:lang="en">A dimension or extent, or a time taken to play or execute.</rdfs:comment>
        <rdfs:isDefinedBy rdf:resource="http://purl.org/dc/terms/"/>
        <rdfs:label xml:lang="en">Size or Duration</rdfs:label>
    </rdf:Description>
    <rdf:Description rdf:about="http://purl.org/dc/terms/Standard">
        <rdfs:comment xml:lang="en">A reference point against which other things can be evaluated or compared.</rdfs:comment>
        <rdfs:isDefinedBy rdf:resource="http://purl.org/dc/terms/"/>
        <rdfs:label xml:lang="en">Standard</rdfs:label>
    </rdf:Description>
    <rdf:Description rdf:about="http://purl.org/dc/terms/URI">
        <rdfs:comment xml:lang="en">The set of identifiers constructed according to the generic syntax for Uniform Resource Identifiers as specified by the Internet Engineering Task Force.</rdfs:comment>
        <rdfs:isDefinedBy rdf:resource="http://purl.org/dc/terms/"/>
        <rdfs:label xml:lang="en">URI</rdfs:label>
        <rdfs:seeAlso rdf:resource="http://www.ietf.org/rfc/rfc3986.txt"/>
    </rdf:Description>
    <rdf:Description rdf:about="http://purl.org/dc/terms/W3CDTF">
        <rdfs:comment xml:lang="en">The set of dates and times constructed according to the W3C Date and Time Formats Specification.</rdfs:comment>
        <rdfs:isDefinedBy rdf:resource="http://purl.org/dc/terms/"/>
        <rdfs:label xml:lang="en">W3C-DTF</rdfs:label>
        <rdfs:seeAlso rdf:resource="http://www.w3.org/TR/NOTE-datetime"/>
    </rdf:Description>
    <rdf:Description rdf:about="http://purl.org/dc/terms/abstract">
        <rdfs:comment xml:lang="en">A summary of the resource.</rdfs:comment>
        <rdfs:isDefinedBy rdf:resource="http://purl.org/dc/terms/"/>
        <rdfs:label xml:lang="en">Abstract</rdfs:label>
    </rdf:Description>
    <rdf:Description rdf:about="http://purl.org/dc/terms/accessRights">
        <dcam:rangeIncludes rdf:resource="http://purl.org/dc/terms/RightsStatement"/>
        <terms:description xml:lang="en">Access Rights may include information regarding access or restrictions based on privacy, security, or other policies.</terms:description>
        <rdfs:comment xml:lang="en">Information about who access the resource or an indication of its security status.</rdfs:comment>
        <rdfs:isDefinedBy rdf:resource="http://purl.org/dc/terms/"/>
        <rdfs:label xml:lang="en">Access Rights</rdfs:label>
    </rdf:Description>
    <rdf:Description rdf:about="http://purl.org/dc/terms/accrualMethod">
        <dcam:rangeIncludes rdf:resource="http://purl.org/dc/terms/MethodOfAccrual"/>
        <terms:description xml:lang="en">Recommended practice is to use a value from the Collection Description Accrual Method Vocabulary [[DCMI-ACCRUALMETHOD](https://dublincore.org/groups/collections/accrual-method/)].</terms:description>
        <rdfs:comment xml:lang="en">The method by which items are added to a collection.</rdfs:comment>
        <rdfs:isDefinedBy rdf:resource="http://purl.org/dc/terms/"/>
        <rdfs:label xml:lang="en">Accrual Method</rdfs:label>
    </rdf:Description>
    <rdf:Description rdf:about="http://purl.org/dc/terms/accrualPeriodicity">
        <dcam:rangeIncludes rdf:resource="http://purl.org/dc/terms/Frequency"/>
        <terms:description xml:lang="en">Recommended practice is to use a value from the Collection Description Frequency Vocabulary [[DCMI-COLLFREQ](https://dublincore.org/groups/collections/frequency/)].</terms:description>
        <rdfs:comment xml:lang="en">The frequency with which items are added to a collection.</rdfs:comment>
        <rdfs:isDefinedBy rdf:resource="http://purl.org/dc/terms/"/>
        <rdfs:label xml:lang="en">Accrual Periodicity</rdfs:label>
    </rdf:Description>
    <rdf:Description rdf:about="http://purl.org/dc/terms/accrualPolicy">
        <dcam:rangeIncludes rdf:resource="http://purl.org/dc/terms/Policy"/>
        <terms:description xml:lang="en">Recommended practice is to use a value from the Collection Description Accrual Policy Vocabulary [[DCMI-ACCRUALPOLICY](https://dublincore.org/groups/collections/accrual-policy/)].</terms:description>
        <rdfs:comment xml:lang="en">The policy governing the addition of items to a collection.</rdfs:comment>
        <rdfs:isDefinedBy rdf:resource="http://purl.org/dc/terms/"/>
        <rdfs:label xml:lang="en">Accrual Policy</rdfs:label>
    </rdf:Description>
    <rdf:Description rdf:about="http://purl.org/dc/terms/alternative">
        <terms:description xml:lang="en">The distinction between titles and alternative titles is application-specific.</terms:description>
        <rdfs:comment xml:lang="en">An alternative name for the resource.</rdfs:comment>
        <rdfs:isDefinedBy rdf:resource="http://purl.org/dc/terms/"/>
        <rdfs:label xml:lang="en">Alternative Title</rdfs:label>
    </rdf:Description>
    <rdf:Description rdf:about="http://purl.org/dc/terms/audience">
        <dcam:rangeIncludes rdf:resource="http://purl.org/dc/terms/AgentClass"/>
        <terms:description xml:lang="en">Recommended practice is to use this property with non-literal values from a vocabulary of audience types.</terms:description>
        <rdfs:comment xml:lang="en">A class of agents for whom the resource is intended or useful.</rdfs:comment>
        <rdfs:isDefinedBy rdf:resource="http://purl.org/dc/terms/"/>
        <rdfs:label xml:lang="en">Audience</rdfs:label>
    </rdf:Description>
    <rdf:Description rdf:about="http://purl.org/dc/terms/available">
        <terms:description xml:lang="en">Recommended practice is to describe the date, date/time, or period of time as recommended for the property Date, of which this is a subproperty.</terms:description>
        <rdfs:comment xml:lang="en">Date that the resource became or will become available.</rdfs:comment>
        <rdfs:isDefinedBy rdf:resource="http://purl.org/dc/terms/"/>
        <rdfs:label xml:lang="en">Date Available</rdfs:label>
    </rdf:Description>
    <rdf:Description rdf:about="http://purl.org/dc/terms/bibliographicCitation">
        <terms:description xml:lang="en">Recommended practice is to include sufficient bibliographic detail to identify the resource as unambiguously as possible.</terms:description>
        <rdfs:comment xml:lang="en">A bibliographic reference for the resource.</rdfs:comment>
        <rdfs:isDefinedBy rdf:resource="http://purl.org/dc/terms/"/>
        <rdfs:label xml:lang="en">Bibliographic Citation</rdfs:label>
    </rdf:Description>
    <rdf:Description rdf:about="http://purl.org/dc/terms/conformsTo">
        <dcam:rangeIncludes rdf:resource="http://purl.org/dc/terms/Standard"/>
        <rdfs:comment xml:lang="en">An established standard to which the described resource conforms.</rdfs:comment>
        <rdfs:isDefinedBy rdf:resource="http://purl.org/dc/terms/"/>
        <rdfs:label xml:lang="en">Conforms To</rdfs:label>
    </rdf:Description>
    <rdf:Description rdf:about="http://purl.org/dc/terms/contributor">
        <dcam:rangeIncludes rdf:resource="http://purl.org/dc/terms/Agent"/>
        <terms:description xml:lang="en">The guidelines for using names of persons or organizations as creators apply to contributors.</terms:description>
        <rdfs:comment xml:lang="en">An entity responsible for making contributions to the resource.</rdfs:comment>
        <rdfs:isDefinedBy rdf:resource="http://purl.org/dc/terms/"/>
        <rdfs:label xml:lang="en">Contributor</rdfs:label>
    </rdf:Description>
    <rdf:Description rdf:about="http://purl.org/dc/terms/coverage">
        <dcam:rangeIncludes rdf:resource="http://purl.org/dc/terms/Jurisdiction"/>
        <dcam:rangeIncludes rdf:resource="http://purl.org/dc/terms/Location"/>
        <dcam:rangeIncludes rdf:resource="http://purl.org/dc/terms/Period"/>
        <terms:description xml:lang="en">Spatial topic and spatial applicability may be a named place or a location specified by its geographic coordinates. Temporal topic may be a named period, date, or date range. A jurisdiction may be a named administrative entity or a geographic place to which the resource applies. Recommended practice is to use a controlled vocabulary such as the Getty Thesaurus of Geographic Names [[TGN](https://www.getty.edu/research/tools/vocabulary/tgn/index.html)]. Where appropriate, named places or time periods may be used in preference to numeric identifiers such as sets of coordinates or date ranges.  Because coverage is so broadly defined, it is preferable to use the more specific subproperties Temporal Coverage and Spatial Coverage.</terms:description>
        <rdfs:comment xml:lang="en">The spatial or temporal topic of the resource, spatial applicability of the resource, or jurisdiction under which the resource is relevant.</rdfs:comment>
        <rdfs:isDefinedBy rdf:resource="http://purl.org/dc/terms/"/>
        <rdfs:label xml:lang="en">Coverage</rdfs:label>
    </rdf:Description>
    <rdf:Description rdf:about="http://purl.org/dc/terms/created">
        <terms:description xml:lang="en">Recommended practice is to describe the date, date/time, or period of time as recommended for the property Date, of which this is a subproperty.</terms:description>
        <rdfs:comment xml:lang="en">Date of creation of the resource.</rdfs:comment>
        <rdfs:isDefinedBy rdf:resource="http://purl.org/dc/terms/"/>
        <rdfs:label xml:lang="en">Date Created</rdfs:label>
    </rdf:Description>
    <rdf:Description rdf:about="http://purl.org/dc/terms/creator">
        <dcam:rangeIncludes rdf:resource="http://purl.org/dc/terms/Agent"/>
        <terms:description xml:lang="en">Recommended practice is to identify the creator with a URI.  If this is not possible or feasible, a literal value that identifies the creator may be provided.</terms:description>
        <rdfs:comment xml:lang="en">An entity responsible for making the resource.</rdfs:comment>
        <rdfs:isDefinedBy rdf:resource="http://purl.org/dc/terms/"/>
        <rdfs:label xml:lang="en">Creator</rdfs:label>
    </rdf:Description>
    <rdf:Description rdf:about="http://purl.org/dc/terms/date">
        <terms:description xml:lang="en">Date may be used to express temporal information at any level of granularity.  Recommended practice is to express the date, date/time, or period of time according to ISO 8601-1 [[ISO 8601-1](https://www.iso.org/iso-8601-date-and-time-format.html)] or a published profile of the ISO standard, such as the W3C Note on Date and Time Formats [[W3CDTF](https://www.w3.org/TR/NOTE-datetime)] or the Extended Date/Time Format Specification [[EDTF](http://www.loc.gov/standards/datetime/)].  If the full date is unknown, month and year (YYYY-MM) or just year (YYYY) may be used. Date ranges may be specified using ISO 8601 period of time specification in which start and end dates are separated by a &apos;/&apos; (slash) character.  Either the start or end date may be missing.</terms:description>
        <rdfs:comment xml:lang="en">A point or period of time associated with an event in the lifecycle of the resource.</rdfs:comment>
        <rdfs:isDefinedBy rdf:resource="http://purl.org/dc/terms/"/>
        <rdfs:label xml:lang="en">Date</rdfs:label>
    </rdf:Description>
    <rdf:Description rdf:about="http://purl.org/dc/terms/dateAccepted">
        <terms:description xml:lang="en">Recommended practice is to describe the date, date/time, or period of time as recommended for the property Date, of which this is a subproperty.  Examples of resources to which a date of acceptance may be relevant are a thesis (accepted by a university department) or an article (accepted by a journal).</terms:description>
        <rdfs:comment xml:lang="en">Date of acceptance of the resource.</rdfs:comment>
        <rdfs:isDefinedBy rdf:resource="http://purl.org/dc/terms/"/>
        <rdfs:label xml:lang="en">Date Accepted</rdfs:label>
    </rdf:Description>
    <rdf:Description rdf:about="http://purl.org/dc/terms/dateCopyrighted">
        <terms:description xml:lang="en">Typically a year.  Recommended practice is to describe the date, date/time, or period of time as recommended for the property Date, of which this is a subproperty.</terms:description>
        <rdfs:comment xml:lang="en">Date of copyright of the resource.</rdfs:comment>
        <rdfs:isDefinedBy rdf:resource="http://purl.org/dc/terms/"/>
        <rdfs:label xml:lang="en">Date Copyrighted</rdfs:label>
    </rdf:Description>
    <rdf:Description rdf:about="http://purl.org/dc/terms/dateSubmitted">
        <terms:description xml:lang="en">Recommended practice is to describe the date, date/time, or period of time as recommended for the property Date, of which this is a subproperty.  Examples of resources to which a &apos;Date Submitted&apos; may be relevant include a thesis (submitted to a university department) or an article (submitted to a journal).</terms:description>
        <rdfs:comment xml:lang="en">Date of submission of the resource.</rdfs:comment>
        <rdfs:isDefinedBy rdf:resource="http://purl.org/dc/terms/"/>
        <rdfs:label xml:lang="en">Date Submitted</rdfs:label>
    </rdf:Description>
    <rdf:Description rdf:about="http://purl.org/dc/terms/description">
        <terms:description xml:lang="en">Description may include but is not limited to: an abstract, a table of contents, a graphical representation, or a free-text account of the resource.</terms:description>
        <rdfs:comment xml:lang="en">An account of the resource.</rdfs:comment>
        <rdfs:isDefinedBy rdf:resource="http://purl.org/dc/terms/"/>
        <rdfs:label xml:lang="en">Description</rdfs:label>
    </rdf:Description>
    <rdf:Description rdf:about="http://purl.org/dc/terms/educationLevel">
        <dcam:rangeIncludes rdf:resource="http://purl.org/dc/terms/AgentClass"/>
        <rdfs:comment xml:lang="en">A class of agents, defined in terms of progression through an educational or training context, for which the described resource is intended.</rdfs:comment>
        <rdfs:isDefinedBy rdf:resource="http://purl.org/dc/terms/"/>
        <rdfs:label xml:lang="en">Audience Education Level</rdfs:label>
    </rdf:Description>
    <rdf:Description rdf:about="http://purl.org/dc/terms/extent">
        <dcam:rangeIncludes rdf:resource="http://purl.org/dc/terms/SizeOrDuration"/>
        <terms:description xml:lang="en">Recommended practice is to specify the file size in megabytes and duration in ISO 8601 format.</terms:description>
        <rdfs:comment xml:lang="en">The size or duration of the resource.</rdfs:comment>
        <rdfs:isDefinedBy rdf:resource="http://purl.org/dc/terms/"/>
        <rdfs:label xml:lang="en">Extent</rdfs:label>
    </rdf:Description>
    <rdf:Description rdf:about="http://purl.org/dc/terms/format">
        <dcam:rangeIncludes rdf:resource="http://purl.org/dc/terms/Extent"/>
        <dcam:rangeIncludes rdf:resource="http://purl.org/dc/terms/MediaType"/>
        <terms:description xml:lang="en">Recommended practice is to use a controlled vocabulary where available. For example, for file formats one could use the list of Internet Media Types [[MIME](https://www.iana.org/assignments/media-types/media-types.xhtml)].  Examples of dimensions include size and duration.</terms:description>
        <rdfs:comment xml:lang="en">The file format, physical medium, or dimensions of the resource.</rdfs:comment>
        <rdfs:isDefinedBy rdf:resource="http://purl.org/dc/terms/"/>
        <rdfs:label xml:lang="en">Format</rdfs:label>
    </rdf:Description>
    <rdf:Description rdf:about="http://purl.org/dc/terms/hasFormat">
        <terms:description xml:lang="en">This property is intended to be used with non-literal values. This property is an inverse property of Is Format Of.</terms:description>
        <rdfs:comment xml:lang="en">A related resource that is substantially the same as the pre-existing described resource, but in another format.</rdfs:comment>
        <rdfs:isDefinedBy rdf:resource="http://purl.org/dc/terms/"/>
        <rdfs:label xml:lang="en">Has Format</rdfs:label>
    </rdf:Description>
    <rdf:Description rdf:about="http://purl.org/dc/terms/hasPart">
        <terms:description xml:lang="en">This property is intended to be used with non-literal values. This property is an inverse property of Is Part Of.</terms:description>
        <rdfs:comment xml:lang="en">A related resource that is included either physically or logically in the described resource.</rdfs:comment>
        <rdfs:isDefinedBy rdf:resource="http://purl.org/dc/terms/"/>
        <rdfs:label xml:lang="en">Has Part</rdfs:label>
    </rdf:Description>
    <rdf:Description rdf:about="http://purl.org/dc/terms/hasVersion">
        <terms:description xml:lang="en">Changes in version imply substantive changes in content rather than differences in format. This property is intended to be used with non-literal values. This property is an inverse property of Is Version Of.</terms:description>
        <rdfs:comment xml:lang="en">A related resource that is a version, edition, or adaptation of the described resource.</rdfs:comment>
        <rdfs:isDefinedBy rdf:resource="http://purl.org/dc/terms/"/>
        <rdfs:label xml:lang="en">Has Version</rdfs:label>
    </rdf:Description>
    <rdf:Description rdf:about="http://purl.org/dc/terms/identifier">
        <terms:description xml:lang="en">Recommended practice is to identify the resource by means of a string conforming to an identification system. Examples include International Standard Book Number (ISBN), Digital Object Identifier (DOI), and Uniform Resource Name (URN).  Persistent identifiers should be provided as HTTP URIs.</terms:description>
        <rdfs:comment xml:lang="en">An unambiguous reference to the resource within a given context.</rdfs:comment>
        <rdfs:isDefinedBy rdf:resource="http://purl.org/dc/terms/"/>
        <rdfs:label xml:lang="en">Identifier</rdfs:label>
    </rdf:Description>
    <rdf:Description rdf:about="http://purl.org/dc/terms/isFormatOf">
        <terms:description xml:lang="en">This property is intended to be used with non-literal values. This property is an inverse property of Has Format.</terms:description>
        <rdfs:comment xml:lang="en">A pre-existing related resource that is substantially the same as the described resource, but in another format.</rdfs:comment>
        <rdfs:isDefinedBy rdf:resource="http://purl.org/dc/terms/"/>
        <rdfs:label xml:lang="en">Is Format Of</rdfs:label>
    </rdf:Description>
    <rdf:Description rdf:about="http://purl.org/dc/terms/isPartOf">
        <terms:description xml:lang="en">This property is intended to be used with non-literal values. This property is an inverse property of Has Part.</terms:description>
        <rdfs:comment xml:lang="en">A related resource in which the described resource is physically or logically included.</rdfs:comment>
        <rdfs:isDefinedBy rdf:resource="http://purl.org/dc/terms/"/>
        <rdfs:label xml:lang="en">Is Part Of</rdfs:label>
    </rdf:Description>
    <rdf:Description rdf:about="http://purl.org/dc/terms/isReferencedBy">
        <terms:description xml:lang="en">This property is intended to be used with non-literal values. This property is an inverse property of References.</terms:description>
        <rdfs:comment xml:lang="en">A related resource that references, cites, or otherwise points to the described resource.</rdfs:comment>
        <rdfs:isDefinedBy rdf:resource="http://purl.org/dc/terms/"/>
        <rdfs:label xml:lang="en">Is Referenced By</rdfs:label>
    </rdf:Description>
    <rdf:Description rdf:about="http://purl.org/dc/terms/isReplacedBy">
        <terms:description xml:lang="en">This property is intended to be used with non-literal values. This property is an inverse property of Replaces.</terms:description>
        <rdfs:comment xml:lang="en">A related resource that supplants, displaces, or supersedes the described resource.</rdfs:comment>
        <rdfs:isDefinedBy rdf:resource="http://purl.org/dc/terms/"/>
        <rdfs:label xml:lang="en">Is Replaced By</rdfs:label>
    </rdf:Description>
    <rdf:Description rdf:about="http://purl.org/dc/terms/isRequiredBy">
        <terms:description xml:lang="en">This property is intended to be used with non-literal values. This property is an inverse property of Requires.</terms:description>
        <rdfs:comment xml:lang="en">A related resource that requires the described resource to support its function, delivery, or coherence.</rdfs:comment>
        <rdfs:isDefinedBy rdf:resource="http://purl.org/dc/terms/"/>
        <rdfs:label xml:lang="en">Is Required By</rdfs:label>
    </rdf:Description>
    <rdf:Description rdf:about="http://purl.org/dc/terms/isVersionOf">
        <terms:description xml:lang="en">Changes in version imply substantive changes in content rather than differences in format. This property is intended to be used with non-literal values. This property is an inverse property of Has Version.</terms:description>
        <rdfs:comment xml:lang="en">A related resource of which the described resource is a version, edition, or adaptation.</rdfs:comment>
        <rdfs:isDefinedBy rdf:resource="http://purl.org/dc/terms/"/>
        <rdfs:label xml:lang="en">Is Version Of</rdfs:label>
    </rdf:Description>
    <rdf:Description rdf:about="http://purl.org/dc/terms/issued">
        <terms:description xml:lang="en">Recommended practice is to describe the date, date/time, or period of time as recommended for the property Date, of which this is a subproperty.</terms:description>
        <rdfs:comment xml:lang="en">Date of formal issuance of the resource.</rdfs:comment>
        <rdfs:isDefinedBy rdf:resource="http://purl.org/dc/terms/"/>
        <rdfs:label xml:lang="en">Date Issued</rdfs:label>
    </rdf:Description>
    <rdf:Description rdf:about="http://purl.org/dc/terms/language">
        <dcam:rangeIncludes rdf:resource="http://purl.org/dc/terms/LinguisticSystem"/>
        <terms:description xml:lang="en">Recommended practice is to use either a non-literal value representing a language from a controlled vocabulary such as ISO 639-2 or ISO 639-3, or a literal value consisting of an IETF Best Current Practice 47 [[IETF-BCP47](https://tools.ietf.org/html/bcp47)] language tag.</terms:description>
        <rdfs:comment xml:lang="en">A language of the resource.</rdfs:comment>
        <rdfs:isDefinedBy rdf:resource="http://purl.org/dc/terms/"/>
        <rdfs:label xml:lang="en">Language</rdfs:label>
    </rdf:Description>
    <rdf:Description rdf:about="http://purl.org/dc/terms/license">
        <dcam:rangeIncludes rdf:resource="http://purl.org/dc/terms/LicenseDocument"/>
        <terms:description xml:lang="en">Recommended practice is to identify the license document with a URI. If this is not possible or feasible, a literal value that identifies the license may be provided.</terms:description>
        <rdfs:comment xml:lang="en">A legal document giving official permission to do something with the resource.</rdfs:comment>
        <rdfs:isDefinedBy rdf:resource="http://purl.org/dc/terms/"/>
        <rdfs:label xml:lang="en">License</rdfs:label>
    </rdf:Description>
    <rdf:Description rdf:about="http://purl.org/dc/terms/mediator">
        <dcam:rangeIncludes rdf:resource="http://purl.org/dc/terms/AgentClass"/>
        <terms:description xml:lang="en">In an educational context, a mediator might be a parent, teacher, teaching assistant, or care-giver.</terms:description>
        <rdfs:comment xml:lang="en">An entity that mediates access to the resource.</rdfs:comment>
        <rdfs:isDefinedBy rdf:resource="http://purl.org/dc/terms/"/>
        <rdfs:label xml:lang="en">Mediator</rdfs:label>
    </rdf:Description>
    <rdf:Description rdf:about="http://purl.org/dc/terms/medium">
        <dcam:domainIncludes rdf:resource="http://purl.org/dc/terms/PhysicalResource"/>
        <dcam:rangeIncludes rdf:resource="http://purl.org/dc/terms/PhysicalMedium"/>
        <rdfs:comment xml:lang="en">The material or physical carrier of the resource.</rdfs:comment>
        <rdfs:isDefinedBy rdf:resource="http://purl.org/dc/terms/"/>
        <rdfs:label xml:lang="en">Medium</rdfs:label>
    </rdf:Description>
    <rdf:Description rdf:about="http://purl.org/dc/terms/modified">
        <terms:description xml:lang="en">Recommended practice is to describe the date, date/time, or period of time as recommended for the property Date, of which this is a subproperty.</terms:description>
        <rdfs:comment xml:lang="en">Date on which the resource was changed.</rdfs:comment>
        <rdfs:isDefinedBy rdf:resource="http://purl.org/dc/terms/"/>
        <rdfs:label xml:lang="en">Date Modified</rdfs:label>
    </rdf:Description>
    <rdf:Description rdf:about="http://purl.org/dc/terms/publisher">
        <dcam:rangeIncludes rdf:resource="http://purl.org/dc/terms/Agent"/>
        <rdfs:comment xml:lang="en">An entity responsible for making the resource available.</rdfs:comment>
        <rdfs:isDefinedBy rdf:resource="http://purl.org/dc/terms/"/>
        <rdfs:label xml:lang="en">Publisher</rdfs:label>
    </rdf:Description>
    <rdf:Description rdf:about="http://purl.org/dc/terms/references">
        <terms:description xml:lang="en">This property is intended to be used with non-literal values. This property is an inverse property of Is Referenced By.</terms:description>
        <rdfs:comment xml:lang="en">A related resource that is referenced, cited, or otherwise pointed to by the described resource.</rdfs:comment>
        <rdfs:isDefinedBy rdf:resource="http://purl.org/dc/terms/"/>
        <rdfs:label xml:lang="en">References</rdfs:label>
    </rdf:Description>
    <rdf:Description rdf:about="http://purl.org/dc/terms/relation">
        <terms:description xml:lang="en">Recommended practice is to identify the related resource by means of a URI.  If this is not possible or feasible, a string conforming to a formal identification system may be provided.</terms:description>
        <rdfs:comment xml:lang="en">A related resource.</rdfs:comment>
        <rdfs:isDefinedBy rdf:resource="http://purl.org/dc/terms/"/>
        <rdfs:label xml:lang="en">Relation</rdfs:label>
    </rdf:Description>
    <rdf:Description rdf:about="http://purl.org/dc/terms/replaces">
        <terms:description xml:lang="en">This property is intended to be used with non-literal values. This property is an inverse property of Is Replaced By.</terms:description>
        <rdfs:comment xml:lang="en">A related resource that is supplanted, displaced, or superseded by the described resource.</rdfs:comment>
        <rdfs:isDefinedBy rdf:resource="http://purl.org/dc/terms/"/>
        <rdfs:label xml:lang="en">Replaces</rdfs:label>
    </rdf:Description>
    <rdf:Description rdf:about="http://purl.org/dc/terms/requires">
        <terms:description xml:lang="en">This property is intended to be used with non-literal values. This property is an inverse property of Is Required By.</terms:description>
        <rdfs:comment xml:lang="en">A related resource that is required by the described resource to support its function, delivery, or coherence.</rdfs:comment>
        <rdfs:isDefinedBy rdf:resource="http://purl.org/dc/terms/"/>
        <rdfs:label xml:lang="en">Requires</rdfs:label>
    </rdf:Description>
    <rdf:Description rdf:about="http://purl.org/dc/terms/rights">
        <dcam:rangeIncludes rdf:resource="http://purl.org/dc/terms/RightsStatement"/>
        <terms:description xml:lang="en">Typically, rights information includes a statement about various property rights associated with the resource, including intellectual property rights.  Recommended practice is to refer to a rights statement with a URI.  If this is not possible or feasible, a literal value (name, label, or short text) may be provided.</terms:description>
        <rdfs:comment xml:lang="en">Information about rights held in and over the resource.</rdfs:comment>
        <rdfs:isDefinedBy rdf:resource="http://purl.org/dc/terms/"/>
        <rdfs:label xml:lang="en">Rights</rdfs:label>
    </rdf:Description>
    <rdf:Description rdf:about="http://purl.org/dc/terms/source">
        <terms:description xml:lang="en">This property is intended to be used with non-literal values. The described resource may be derived from the related resource in whole or in part. Best practice is to identify the related resource by means of a URI or a string conforming to a formal identification system.</terms:description>
        <rdfs:comment xml:lang="en">A related resource from which the described resource is derived.</rdfs:comment>
        <rdfs:isDefinedBy rdf:resource="http://purl.org/dc/terms/"/>
        <rdfs:label xml:lang="en">Source</rdfs:label>
    </rdf:Description>
    <rdf:Description rdf:about="http://purl.org/dc/terms/spatial">
        <dcam:rangeIncludes rdf:resource="http://purl.org/dc/terms/Location"/>
        <rdfs:comment xml:lang="en">Spatial characteristics of the resource.</rdfs:comment>
        <rdfs:isDefinedBy rdf:resource="http://purl.org/dc/terms/"/>
        <rdfs:label xml:lang="en">Spatial Coverage</rdfs:label>
    </rdf:Description>
    <rdf:Description rdf:about="http://purl.org/dc/terms/subject">
        <terms:description xml:lang="en">Recommended practice is to refer to the subject with a URI. If this is not possible or feasible, a literal value that identifies the subject may be provided. Both should preferably refer to a subject in a controlled vocabulary.</terms:description>
        <rdfs:comment xml:lang="en">A topic of the resource.</rdfs:comment>
        <rdfs:isDefinedBy rdf:resource="http://purl.org/dc/terms/"/>
        <rdfs:label xml:lang="en">Subject</rdfs:label>
    </rdf:Description>
    <rdf:Description rdf:about="http://purl.org/dc/terms/tableOfContents">
        <rdfs:comment xml:lang="en">A list of subunits of the resource.</rdfs:comment>
        <rdfs:isDefinedBy rdf:resource="http://purl.org/dc/terms/"/>
        <rdfs:label xml:lang="en">Table Of Contents</rdfs:label>
    </rdf:Description>
    <rdf:Description rdf:about="http://purl.org/dc/terms/temporal">
        <dcam:rangeIncludes rdf:resource="http://purl.org/dc/terms/PeriodOfTime"/>
        <rdfs:comment xml:lang="en">Temporal characteristics of the resource.</rdfs:comment>
        <rdfs:isDefinedBy rdf:resource="http://purl.org/dc/terms/"/>
        <rdfs:label xml:lang="en">Temporal Coverage</rdfs:label>
    </rdf:Description>
    <rdf:Description rdf:about="http://purl.org/dc/terms/title">
        <rdfs:comment xml:lang="en">A name given to the resource.</rdfs:comment>
        <rdfs:isDefinedBy rdf:resource="http://purl.org/dc/terms/"/>
        <rdfs:label xml:lang="en">Title</rdfs:label>
    </rdf:Description>
    <rdf:Description rdf:about="http://purl.org/dc/terms/type">
        <terms:description xml:lang="en">Recommended practice is to use a controlled vocabulary such as the DCMI Type Vocabulary [[DCMI-TYPE](http://dublincore.org/documents/dcmi-type-vocabulary/)]. To describe the file format, physical medium, or dimensions of the resource, use the property Format.</terms:description>
        <rdfs:comment xml:lang="en">The nature or genre of the resource.</rdfs:comment>
        <rdfs:isDefinedBy rdf:resource="http://purl.org/dc/terms/"/>
        <rdfs:label xml:lang="en">Type</rdfs:label>
    </rdf:Description>
    <rdf:Description rdf:about="http://purl.org/dc/terms/valid">
        <terms:description xml:lang="en">Recommended practice is to describe the date, date/time, or period of time as recommended for the property Date, of which this is a subproperty.</terms:description>
        <rdfs:comment xml:lang="en">Date (often a range) of validity of a resource.</rdfs:comment>
        <rdfs:isDefinedBy rdf:resource="http://purl.org/dc/terms/"/>
        <rdfs:label xml:lang="en">Date Valid</rdfs:label>
    </rdf:Description>
</rdf:RDF>



<!-- Generated by the OWL API (version 5.1.18) https://github.com/owlcs/owlapi/ -->


